examples/containers/theories/MapProofs/DeleteUpdateProofs.v
@@ -1,0 +1,406 @@
+Require Import GHC.Base.
+Import GHC.Base.Notations.
+Require Import Proofs.GHC.Base.
+Require Import Data.Map.Internal.
+Import GHC.Num.Notations.
+Require Import OrdTactic.
+Require Import Psatz.
+Require Import Tactics.
+Set Bullet Behavior "Strict Subproofs".
+Require Import MapProofs.Bounds.
+Require Import MapProofs.Tactics.
+Require Import MapProofs.MaxMinProofs.
+Require Import MapProofs.InsertProofs.
+
+Section WF.
+Context {e : Type} {a : Type} {HEq : Eq_ e} {HOrd : Ord e} {HEqLaws : EqLaws e}  {HOrdLaws : OrdLaws e}.
+
+(** ** Verification of [glue] *)
+
+Lemma glue_Desc:
+  forall (s1: Map e a) s2 lb ub x,
+  Bounded s1 lb (Some x) ->
+  Bounded s2 (Some x) ub ->
+  isLB lb x = true ->
+  isUB ub x = true ->
+  balance_prop (size s1) (size s2) ->
+  Desc (glue s1 s2) lb ub ((size s1 + size s2)%Z) (fun i => sem s1 i ||| sem s2 i).
+Proof.
+  intros ????? HB1 HB2 ???.
+
+  inversion HB1; inversion HB2; subst; cbn -[Z.add]; clear HB1 HB2.
+  1-3: solve [solve_Desc e|solve_size].
+  destruct (Z.ltb_spec (1 + size s4 + size s5) (1 + size s0 + size s3)).
+  - eapply maxViewSure_Desc; only 1: solve_Bounded e.
+    intros y vy r [Hthere HD].
+    applyDesc e HD.
+    destruct Hthere as [[??]|Hthere].
+      (*TODO: See why this is not rewriting automatically*)
+    * subst. applyDesc e (@balanceR_Desc e a). rewrite size_Bin in *. rewrite size_Bin in H1.
+      solve_size. solve_Desc e. repeat(rewrite size_Bin in H1). rewrite size_Bin in Hsz0. solve_size.
+      (*subst; applyDesc e (@balanceR_Desc e a); solve_Desc e.*)
+    * subst; applyDesc e (@balanceR_Desc e a). rewrite size_Bin in *. rewrite size_Bin in H1. solve_size.
+      solve_Desc e. rewrite size_Bin in Hsz0. solve_size.
+  - eapply minViewSure_Desc; only 1: solve_Bounded e.
+    intros y vy r [Hthere HD].
+    applyDesc e HD.
+    destruct Hthere as [[??]|Hthere]; subst; applyDesc e (@balanceL_Desc e a).
+    rewrite size_Bin in H1. solve_size. solve_Desc e. rewrite size_Bin in Hsz0. solve_size.
+    rewrite size_Bin in H1. solve_size. solve_Desc e. rewrite size_Bin in Hsz0. solve_size.
+    
+Qed.
+
+(** ** Verification of [delete] *)
+
+Lemma delete_Desc :
+  forall x (s: Map e a) lb ub,
+  Bounded s lb ub ->
+  Desc (delete x s) lb ub (if isSome (sem s x) then (size s - 1) else size s) (fun i => if i == x then None else sem s i).
+Proof.
+  intros ???? HB.
+  induction HB; intros; subst.
+  - simpl. solve_Desc e.
+  - cbn -[Z.add].
+    destruct (compare x x0) eqn:Heq.
+    + replace (x == x0) with true by solve_Bounds e.
+      simpl_options.
+      applyDesc e glue_Desc.
+      solve_Desc e.
+    + applyDesc e IHHB1; clear IHHB1 IHHB2.
+      replace (x == x0) with false by solve_Bounds e.
+      rewrite -> (sem_outside_below HB2) by solve_Bounds e.
+      simpl_options.
+      destruct_ptrEq.
+      * replace (isSome (sem s1 x)) with false in *
+          by (destruct (sem s1 x); simpl in *;  try congruence; lia).
+        solve_Desc e.
+      * destruct (sem s1 x); cbn -[Z.add] in *; applyDesc e (@balanceR_Desc e a); solve_Desc e.
+    + applyDesc e IHHB2; clear IHHB1 IHHB2.
+      replace (x == x0) with false by solve_Bounds e.
+      rewrite -> (sem_outside_above HB1) by solve_Bounds e.
+      simpl_options.
+      destruct_ptrEq.
+      * replace (isSome (sem s2 x)) with false by (destruct (sem s2 x); simpl in *; try congruence; lia).
+        solve_Desc e.
+      * destruct (sem s2 x); cbn -[Z.add] in *; applyDesc e (@balanceL_Desc e a); solve_Desc e.
+Qed.
+
+(** ** Verification of [deleteMin] *)
+
+(** It is hard to phrase this without refering to [lookupMin] *)
+
+Lemma deleteMin_Desc :
+  forall (m: Map e a) lb ub,
+  Bounded m lb ub ->
+  deleteMin m = match lookupMin m with | None => m
+                                       | Some (x, y) => delete x m end.
+Proof.
+  intros ??? HD.
+  induction HD.
+  * reflexivity.
+  * clear IHHD2.
+    cbn [deleteMin].
+    rewrite IHHD1; clear IHHD1.
+
+    destruct s1 eqn:?.
+    + replace (lookupMin (Bin sz x v (Bin s e0 a0 m1 m2) s2)) with (lookupMin (Bin s e0 a0 m1 m2)) by reflexivity.
+      rewrite <- Heqm in *. clear  s e0 a0 m1 m1 Heqm.
+
+      pose proof (lookupMin_Desc s1 lb (Some x) HD1) as Hlookup.
+      destruct (lookupMin s1) as [ex|].
+      - destruct ex. destruct Hlookup as [Hthere Hextrem].
+        simpl.
+        apply (sem_inside HD1) in Hthere. destruct Hthere.
+        replace (compare e0 x) with Lt by (symmetry; solve_Bounds e).
+        ** destruct_ptrEq.
+           ++ rewrite Hpe. clear Hpe.
+              eapply balanceR_noop; try eassumption.
+           ++ reflexivity.
+       - rewrite H1.
+          eapply balanceR_noop; try eassumption.
+   + simpl.
+     replace (compare x x) with Eq by (symmetry; order e).
+     reflexivity.
+Qed.
+
+(** ** Verification of [deleteMax] *)
+
+(** It is hard to phrase this without refering to [lookupMax] *)
+
+Lemma deleteMax_Desc :
+  forall (m: Map e a) lb ub,
+  Bounded m lb ub ->
+  deleteMax m = match lookupMax m with | None => m
+                                       | Some (x, y) => delete x m end.
+Proof.
+  intros ??? HD.
+  induction HD.
+  * reflexivity.
+  * clear IHHD1.
+    cbn [deleteMax].
+    rewrite IHHD2; clear IHHD2.
+
+    destruct s2 eqn:?.
+    + replace (lookupMax (Bin sz x v s1 (Bin s e0 a0 m1 m2))) with (lookupMax (Bin s e0 a0 m1 m2)) by reflexivity.
+      rewrite <- Heqm in *. clear s e0 a0 m1 m2 Heqm.
+
+      pose proof (lookupMax_Desc s2 (Some x) ub HD2) as Hlookup.
+      destruct (lookupMax s2) as [ex|].
+      - destruct ex. destruct Hlookup as [Hthere Hextrem].
+        simpl.
+        apply (sem_inside HD2) in Hthere. destruct Hthere.
+        replace (compare e0 x) with Gt by (symmetry; solve_Bounds e).
+        ** destruct_ptrEq.
+           ++ rewrite Hpe. clear Hpe.
+              eapply balanceL_noop; try eassumption.
+           ++ reflexivity.
+       - rewrite H1.
+          eapply balanceL_noop; try eassumption.
+   + simpl.
+     replace (compare x x) with Eq by (symmetry; order e).
+     destruct s1; reflexivity.
+Qed.
+
+(** ** Verification of [adjustWithKey *)
+Require Import Coq.Classes.Morphisms. (* For [Proper] *)
+
+(*TODO: Had to add assumption that f is proper*)
+Lemma adjustWithKey_Desc :
+  forall x f (m: Map e a) lb ub,
+  Bounded m lb ub ->
+  Proper ((fun i j : e => _GHC.Base.==_ i j = true) ==> eq) f ->
+  Desc (adjustWithKey f x m) lb ub (size m) (fun i => if i == x then match (sem m x) with
+                                                                     | Some v => Some (f x v)
+                                                                     | None => None end else sem m i).
+Proof.
+  intros ????? HA HP. induction HA.
+  - simpl. solve_Desc e.
+  - cbn -[Z.add]. destruct (compare x x0) eqn : ?.
+    + replace (x == x0) with true by solve_Bounds e. simpl_options.
+      solve_Desc e. f_solver e.
+      assert (f x0 v = f x v). apply equal_f. apply HP. order e. rewrite H3. reflexivity.
+    + applyDesc e IHHA1; clear IHHA1 IHHA2. replace (x == x0) with false by solve_Bounds e.
+      rewrite -> (sem_outside_below HA2) by solve_Bounds e.
+      simpl_options. solve_Desc e. 
+    + applyDesc e IHHA2; clear IHHA1 IHHA2. replace (x == x0) with false by solve_Bounds e.
+      rewrite -> (sem_outside_above HA1) by solve_Bounds e. simpl_options.
+      solve_Desc e.
+Qed.
+
+(** ** Verification of [adjust] *)
+Lemma adjust_spec: forall (m: Map e a) (f: a -> a) k,
+  adjust f k m = adjustWithKey (fun _ x => f x) k m.
+Proof. 
+  intros. unfold adjust. reflexivity.
+Qed.
+
+(** ** Verification of [updateWithKey] *)
+Lemma updateWithKey_Desc:
+  forall x f (m: Map e a) lb ub,
+  Bounded m lb ub ->
+  Proper ((fun i j : e => _GHC.Base.==_ i j = true) ==> eq) f ->
+  Desc (updateWithKey f x m) lb ub (match sem m x with
+                                    | None => size m
+                                    | Some y => if isSome (f x y) then
+                                       size m else size m - 1
+                                      end) (fun i => if i == x then match (sem m x) with
+                                                                     | Some v => f x v
+                                                                     | None => None end else sem m i).
+Proof.
+intros ????? HB HP.
+  induction HB; intros; subst.
+  - simpl. solve_Desc e.
+  - cbn -[Z.add].
+    destruct (compare x x0) eqn:Heq.
+    + assert (f x0 v = f x v). apply equal_f. apply HP. order e.
+      replace (x == x0) with true by solve_Bounds e.
+      simpl_options. destruct (f x0 v) eqn : ?.
+      * solve_Desc e. rewrite size_Bin in *.
+        rewrite -> (sem_outside_above HB1) by solve_Bounds e.
+        rewrite -> (sem_outside_below HB2) by solve_Bounds e.
+        simpl_options. rewrite <- H1. reflexivity. 
+      * applyDesc e glue_Desc. solve_Desc e. 
+        rewrite -> (sem_outside_above HB1) by solve_Bounds e.
+        rewrite -> (sem_outside_below HB2) by solve_Bounds e.
+        simpl_options. rewrite <-H1. cbn -[Z.add]. rewrite Hsz. omega.
+    + applyDesc e IHHB1. replace (x == x0) with false by solve_Bounds e.
+      rewrite -> (sem_outside_below HB2) by solve_Bounds e.
+      simpl_options. destruct (sem s1 x); cbn -[Z.add] in *; applyDesc e (@balanceR_Desc e a).
+      destruct (f x a0) eqn : ?. simpl in Hsz. rewrite Hsz. left. assumption.
+      simpl in Hsz. rewrite Hsz. solve_size.
+      solve_Desc e. rewrite Hsz0. destruct (f x a0); simpl in Hsz; rewrite Hsz;
+      cbn -[Z.add]. reflexivity. omega. solve_Desc e.
+    + applyDesc e IHHB2. replace (x == x0) with false by (order e). 
+      rewrite -> (sem_outside_above HB1) by solve_Bounds e.
+      simpl_options. destruct (sem s2 x); cbn -[Z.add] in *; applyDesc e (@balanceL_Desc e a).
+      destruct (f x a0) eqn : ?. simpl in Hsz. rewrite Hsz. left. assumption.
+      simpl in Hsz. rewrite Hsz. solve_size.
+      solve_Desc e. rewrite Hsz0. destruct (f x a0); simpl in Hsz; rewrite Hsz; cbn -[Z.add]; omega.
+      solve_Desc e.
+Qed.
+
+(** ** Verification of [update] *)
+Lemma update_spec: forall (m: Map e a) (f: a -> option a) k,
+  update f k m = updateWithKey (fun _ x => f x) k m.
+Proof. 
+  intros. unfold update. reflexivity.
+Qed.
+
+(** ** Verification of [updateLookupWithKey] *)
+Lemma updateLookupWithKey_lookup_f_true:
+  forall (m: Map e a) lb ub f k v v1,
+  Bounded m lb ub ->
+  Proper ((fun i j : e => _GHC.Base.==_ i j = true) ==> eq) f ->
+  sem m k = Some v ->
+  f k v = Some v1 ->
+  fst ((updateLookupWithKey f k m)) = Some v1.
+Proof.
+  intros. generalize dependent k. revert v v1. induction H; intros.
+  - inversion H1.
+  - simpl. simpl in H6. destruct (sem s1 k) eqn : ?.
+   + assert (compare k x = Lt) by (solve_Bounds e). rewrite H8. 
+     rewrite (pair_fst_snd (updateLookupWithKey f k s1 )). simpl.
+     eapply IHBounded1. apply Heqo. inversion H6. apply H7.
+   + simpl in H6. destruct (k == x) eqn : ?.
+      * simpl in H6. assert (compare k x = Eq) by (order e).
+        rewrite H8. destruct (f x v) eqn : ?.
+        -- simpl. inversion H6; subst. rewrite <- Heqo0. rewrite <- H7.
+           apply equal_f. apply H0. order e.
+        -- simpl. inversion H6; subst. assert (f k v0 = f x v0). apply equal_f.
+           apply H0. order e. rewrite <- H4 in Heqo0. rewrite Heqo0 in H7.
+           inversion H7.
+      * simpl. destruct (sem s2 k) eqn : ?.
+        -- assert (compare k x = Gt) by (solve_Bounds e). rewrite H8. 
+           rewrite (pair_fst_snd (updateLookupWithKey f k s2 )). simpl.
+           eapply IHBounded2. apply Heqo0. inversion H6; subst. apply H7.
+        -- inversion H6.
+Qed.
+
+Lemma updateLookupWithKey_lookup_f_false:
+  forall (m: Map e a) lb ub f k v,
+  Bounded m lb ub ->
+  Proper ((fun i j : e => _GHC.Base.==_ i j = true) ==> eq) f ->
+  sem m k = Some v ->
+  f k v = None ->
+  fst ((updateLookupWithKey f k m)) = Some v.
+Proof.
+  intros. generalize dependent v. revert k. induction H; intros.
+  - inversion H1.
+  - simpl in H6. simpl. destruct (sem s1 k) eqn : ?.
+    + assert (compare k x = Lt) by (solve_Bounds e). rewrite H8.
+      rewrite (pair_fst_snd (updateLookupWithKey f k s1 )). simpl.
+      eapply IHBounded1. inversion H6; subst. apply Heqo. apply H7.
+    + simpl in H6. destruct (k == x) eqn : ?.
+      * simpl in H6. assert (compare k x = Eq) by (order e).
+        rewrite H8. destruct (f x v) eqn : ?.
+        -- simpl. inversion H6; subst.  assert (f k v0 = f x v0). apply equal_f.
+           apply H0. order e. rewrite H4 in H7. rewrite H7 in Heqo0. inversion Heqo0.
+        -- simpl. assumption.
+      * simpl in H6. assert (compare k x = Gt) by (solve_Bounds e). rewrite H8. 
+           rewrite (pair_fst_snd (updateLookupWithKey f k s2 )). simpl.
+           eapply IHBounded2. apply H6. apply H7.
+Qed. 
+
+Lemma updateLookupWithKey_lookup_None:
+  forall (m: Map e a) lb ub f k,
+  Bounded m lb ub ->
+  Proper ((fun i j : e => _GHC.Base.==_ i j = true) ==> eq) f ->
+  sem m k = None ->
+  fst ((updateLookupWithKey f k m)) = None.
+Proof.
+  intros. generalize dependent k. induction H; intros.
+  - simpl. reflexivity.
+  - simpl in H6. simpl. destruct (sem s1 k) eqn : ?. inversion H6.
+    destruct (k == x) eqn : ?. inversion H6. destruct (sem s2 k) eqn : ?.
+    inversion H6.
+    destruct (compare k x) eqn : ?.
+    + order e.
+    + rewrite (pair_fst_snd (updateLookupWithKey f k s1 )). simpl. apply IHBounded1.
+      assumption.
+    + rewrite (pair_fst_snd (updateLookupWithKey f k s2 )). simpl. apply IHBounded2.
+      assumption.
+Qed.
+
+(*This makes the Desc incredibly easy*)
+Lemma updateWithKey_updateLookupWithKey: forall (m: Map e a) f k,
+  updateWithKey f k m = snd(updateLookupWithKey f k m).
+Proof.
+  intros m. induction m; intros.
+  - simpl. destruct (compare k0 k).
+    + destruct (f k a0); simpl; reflexivity. 
+    + rewrite (pair_fst_snd (updateLookupWithKey f k0 m1)). simpl.
+      rewrite IHm1. reflexivity.
+    + rewrite (pair_fst_snd (updateLookupWithKey f k0 m2)). simpl.
+      rewrite IHm2. reflexivity.
+  - simpl. reflexivity.
+Qed.  
+
+Lemma updateLookupWithKey_Desc: 
+  forall x f (m: Map e a) lb ub,
+  Bounded m lb ub ->
+  Proper ((fun i j : e => _GHC.Base.==_ i j = true) ==> eq) f ->
+  Desc (snd(updateLookupWithKey f x m)) lb ub (match sem m x with
+                                    | None => size m
+                                    | Some y => if isSome (f x y) then
+                                       size m else size m - 1
+                                      end) (fun i => if i == x then match (sem m x) with
+                                                                     | Some v => f x v
+                                                                     | None => None end else sem m i).
+Proof.
+  intros. rewrite <- updateWithKey_updateLookupWithKey. apply updateWithKey_Desc; assumption.
+Qed.
+
+
+(** ** Verification of [alter] *)
+(*Note: the bounds assumptions are only needed in the insert case, but we can always expand the bounds
+  if needed*)
+Lemma alter_Desc:
+  forall m (f: option a -> option a) k lb ub,
+  Bounded m lb ub ->
+  isLB lb k = true ->
+  isUB ub k = true ->
+  Desc(alter f k m) lb ub (if (negb (isSome (sem m k)) && isSome (f None)) then (1 + size m)%Z
+  else if (isSome(sem m k) && negb (isSome (f (sem m k)))) then (size m - 1)%Z else size m)
+  (fun i => (if i == k then f (sem m k) else sem m i)).
+Proof.
+  intros ????? HB HL HU. induction HB.
+  - simpl. destruct (f None).
+    + applyDesc e (@singleton_Desc e a). solve_Desc e.
+    + solve_Desc e.
+  - cbn -[Z.add]. destruct (compare k x) eqn : Heq.
+    + replace (k == x) with true by solve_Bounds e. simpl_options.
+      destruct (f (Some v)) eqn : ?.
+      * solve_Desc e. simpl. 
+        rewrite -> (sem_outside_above HB1) by (solve_Bounds e). simpl_options.
+        rewrite Heqo. simpl. reflexivity. f_solver e.
+        assert (sem s1 k = None). eapply sem_outside_above. eassumption.
+        solve_Bounds e. rewrite H3 in Heqo1. simpl in Heqo1. rewrite Heqo1 in Heqo.
+        inversion Heqo. reflexivity.
+        assert (sem s1 k = None). eapply sem_outside_above. eassumption. solve_Bounds e.
+        rewrite H3 in Heqo1. simpl in Heqo1. rewrite Heqo1 in Heqo. inversion Heqo.
+      * rewrite -> (sem_outside_above HB1) by (solve_Bounds e).
+        rewrite -> (sem_outside_below HB2) by (solve_Bounds e).
+        simpl_options. applyDesc e glue_Desc. solve_Desc e.
+        simpl. rewrite Heqo. simpl. solve_size.
+    + replace (k == x) with false by solve_Bounds e. 
+      rewrite -> (sem_outside_below HB2) by (solve_Bounds e).
+      simpl_options.
+      applyDesc e IHHB1. applyDesc e (@balance_Desc e a). destruct (sem s1 k). simpl in Hsz.
+      destruct (f (Some a0)); simpl in Hsz; solve_size. cbn -[Z.add] in *.
+      destruct (f None). cbn -[Z.add] in *. solve_size.
+      simpl in Hsz. solve_size. solve_Desc e.
+      rewrite Hsz0. rewrite Hsz. destruct (sem s1 k); cbn -[Z.add].
+      destruct (f(Some a0)); cbn -[Z.add]; solve_size.
+      destruct (f(None)); cbn -[Z.add]; solve_size.
+    + replace (k == x) with false by (order e).
+      rewrite -> (sem_outside_above HB1) by (solve_Bounds e). 
+      simpl_options.
+      applyDesc e IHHB2. applyDesc e (@balance_Desc e a). destruct (sem s2 k); cbn -[Z.add] in *.
+      destruct (f(Some a0)); cbn -[Z.add] in *; solve_size.
+      destruct (f(None)); cbn -[Z.add] in *; solve_size.
+      solve_Desc e. rewrite Hsz0. rewrite Hsz. destruct (sem s2 k); cbn -[Z.add].
+      destruct (f(Some a0)); cbn -[Z.add]; solve_size.
+      destruct (f(None)); cbn -[Z.add]; solve_size.
+Qed.
+
+End WF.
