examples/containers/theories/MapProofs/FromListProofs.v
@@ -1,0 +1,1844 @@
+Require Import GHC.Base.
+Import GHC.Base.Notations.
+Require Import Proofs.GHC.Base.
+Require Import Data.Map.Internal.
+Import GHC.Num.Notations.
+Require Import OrdTactic.
+Require Import Psatz.
+Require Import Tactics.
+Set Bullet Behavior "Strict Subproofs".
+Require Import MapProofs.Bounds.
+Require Import MapProofs.Tactics.
+Require Import MapProofs.InsertProofs.
+
+Section WF.
+Context {e : Type} {a : Type} {HEq : Eq_ e} {HOrd : Ord e} {HEqLaws : EqLaws e}  {HOrdLaws : OrdLaws e}.
+
+(** ** Verification of [fromDistinctAscList] *)
+
+Require Import GHC.DeferredFix.
+
+Definition fromDistinctAscList_create_f : (Int -> list (e * a) -> (Map e a) * list (e * a)) -> 
+(Int -> list (e * a) -> Map e a * list ( e * a)).
+Proof.
+  let rhs := eval unfold fromDistinctAscList in (@fromDistinctAscList e a) in
+  lazymatch rhs with context [deferredFix2 ?f] => exact f end.
+Defined.
+
+Definition fromDistinctAscList_create : Int -> list (e * a) -> (Map e a) * list (e * a)
+  := deferredFix2 (fromDistinctAscList_create_f).
+
+Lemma Z_shiftr_pos:
+  forall x, (1 < x -> 1 <= Z.shiftr x 1)%Z.
+Proof.
+  intros.
+  rewrite Z.shiftr_div_pow2 by lia.
+  replace (2^1)%Z with 2%Z by reflexivity.
+  assert (2 <= x)%Z by lia. clear H.
+  apply Z.div_le_mono with (c := 2%Z) in H0.
+  apply H0.
+  lia.
+Qed.
+
+Lemma Z_shiftl_pos:
+  forall x, (1 <= x -> 1 <= Z.shiftl x 1)%Z.
+Proof.
+  intros.
+  rewrite Z.shiftl_mul_pow2 by lia.
+  lia.
+Qed.
+
+Lemma Z_shiftr_lt:
+  forall x, (1 <= x -> Z.shiftr x 1 < x)%Z.
+Proof.
+  intros.
+  rewrite Z.shiftr_div_pow2 by lia.
+  replace (2^1)%Z with 2%Z by reflexivity.
+  apply Z_div_lt; lia.
+Qed.
+
+Require Import Coq.Wellfounded.Wellfounded.
+
+Lemma fromDistinctAscList_create_eq:
+  forall i xs, (1 <= i)%Z ->
+  fromDistinctAscList_create i xs = fromDistinctAscList_create_f fromDistinctAscList_create i xs.
+Proof.
+  intros.
+  change (uncurry fromDistinctAscList_create (i, xs) = uncurry (fromDistinctAscList_create_f fromDistinctAscList_create) (i, xs)).
+  apply deferredFix_eq_on with
+    (f := fun g => uncurry (fromDistinctAscList_create_f (curry g)))
+    (P := fun p => (1 <= fst p)%Z)
+    (R := fun x y => (1 <= fst x < fst y)%Z).
+  * eapply wf_inverse_image with (R := fun x y => (1 <= x < y)%Z).
+    apply Z.lt_wf with (z := 1%Z).
+  * clear i xs H.
+    intros g h x Px Heq.
+    destruct x as [i xs]. simpl in *.
+    unfold fromDistinctAscList_create_f.
+    destruct_match; try reflexivity.
+    repeat replace (#1) with 1%Z by reflexivity.
+    unfold op_zeze__, Eq_Integer___, op_zeze____.
+    destruct (Z.eqb_spec i 1); try reflexivity.
+    unfold curry.
+    assert (1 < i)%Z by lia.
+    assert (1 <= Z.shiftr i 1)%Z by (apply Z_shiftr_pos; lia).
+    assert (Z.shiftr i 1 < i)%Z by (apply Z_shiftr_lt; lia).
+    repeat expand_pairs. simpl.
+    rewrite Heq by eauto.
+    destruct_match; try reflexivity.
+    rewrite Heq by eauto.
+    reflexivity.
+  * simpl; lia.
+Qed.
+
+Check length.
+(* We need to know that [create] returns no longer list than it receives. *)
+Program Fixpoint fromDistinctAscList_create_preserves_length
+  i xs {measure (Z.to_nat i)} :
+  (1 <= i)%Z ->
+  forall (P : Map e a * list (e * a) -> Prop),
+  ( forall s ys,
+    (length ys <= length xs)%nat ->
+    P (s, ys)
+  ) ->
+  P (fromDistinctAscList_create i xs) := _.
+Next Obligation.
+  intros.
+  rename fromDistinctAscList_create_preserves_length into IH.
+  rewrite fromDistinctAscList_create_eq by assumption.
+  unfold fromDistinctAscList_create_f.
+  destruct xs.
+  * apply H0. reflexivity.
+  * repeat replace (#1) with 1%Z by reflexivity.
+    unfold op_zeze__, Eq_Integer___, op_zeze____.
+    destruct (Z.eqb_spec i 1).
+    + destruct p. apply H0. simpl. lia.
+    + assert (Z.to_nat (Bits.shiftR i #1) < Z.to_nat i)%nat. {
+        apply Z2Nat.inj_lt.
+        apply Z.shiftr_nonneg. lia.
+        lia.
+        apply Z_shiftr_lt; lia.
+      }
+      apply IH.
+      - assumption. 
+      - apply Z_shiftr_pos; lia.
+      - intros.
+        destruct_match.
+        ** apply H0. simpl in *. lia.
+        ** apply IH.
+           -- assumption.
+           -- apply Z_shiftr_pos; lia.
+           -- intros.
+               destruct p0. apply H0. simpl in *. lia.
+Qed.
+
+Definition fromDistinctAscList_go_f : (Int -> Map e a -> list (e * a) -> Map e a) ->
+ (Int -> Map e a -> list (e * a) -> Map e a).
+Proof.
+  let rhs := eval unfold fromDistinctAscList in (@fromDistinctAscList e a) in
+  let rhs := eval fold fromDistinctAscList_create_f in rhs in 
+  let rhs := eval fold fromDistinctAscList_create in rhs in 
+  lazymatch rhs with context [deferredFix3 ?f] => exact f end.
+Defined.
+
+Definition fromDistinctAscList_go : Int -> Map e a -> list (e * a) -> Map e a
+  := deferredFix3 (fromDistinctAscList_go_f).
+
+Lemma fromDistinctAscList_go_eq:
+  forall i s xs, (0 < i)%Z ->
+  fromDistinctAscList_go i s xs = fromDistinctAscList_go_f fromDistinctAscList_go i s xs.
+Proof.
+  intros.
+  change (deferredFix (fun g => uncurry (uncurry (fromDistinctAscList_go_f (curry (curry g))))) (i, s, xs) =
+    uncurry (uncurry (fromDistinctAscList_go_f fromDistinctAscList_go)) (i, s, xs)).
+  rewrite deferredFix_eq_on with
+    (P := fun p => (1 <= fst (fst p))%Z)
+    (R := fun x y => (length (snd x) < length (snd y))%nat); only 1: reflexivity.
+  * apply well_founded_ltof with (f := fun x => length (snd x)).
+  * intros g h p Px Heq.
+    destruct p as [[x y] z].
+    simpl in *.
+    unfold fromDistinctAscList_go_f.
+    destruct_match; try reflexivity.
+    eapply fromDistinctAscList_create_preserves_length; try lia.
+    intros s' ys Hlength. destruct p.
+    apply Heq.
+    + apply Z_shiftl_pos.
+      lia.
+    + simpl. lia.
+  * simpl. lia.
+Qed.
+
+Definition safeHd {a} : list (e * a) -> option e := fun xs =>
+  match xs with nil => None | ((x, y)::_) => Some x end.
+
+Lemma mul_pow_sub:
+  forall sz, (0 < sz)%Z -> (2 * 2 ^ (sz - 1) = 2^sz)%Z.
+Proof.
+  intros.
+  rewrite <- Z.pow_succ_r by lia.
+  f_equal.
+  lia.
+Qed.
+
+Require Import Coq.Sorting.Sorted.
+Require Import SortedUtil.
+
+(*Maps are sorted only by keys*)
+Local Definition lt : e * a -> e * a -> Prop
+  := fun x1 x2 => let (e1, a1) := x1 in let (e2, a2) := x2 in (e1 < e2) = true.
+
+(*TODO: FIGURE OUT WHY THIS IS NOT WORKING*)
+Program Fixpoint fromDistinctAscList_create_Desc
+  sz lb xs x {measure (Z.to_nat sz)} :
+  (0 <= sz)%Z ->
+  StronglySorted lt ((lb, x) :: xs) ->
+  forall (P : (Map e a) * list (e * a) -> Prop),
+  ( forall (s : Map e a) (ys: list (e * a)),
+    Bounded s (Some lb) (safeHd ys) ->
+    xs = toList s ++ ys ->
+    ys = nil \/ size s = (2*2^sz-1)%Z ->
+    P (s, ys)
+  ) ->
+  P (fromDistinctAscList_create (2^sz)%Z xs) := _.
+Next Obligation.
+  intros ????? Hnonneg HSorted.  
+  rename fromDistinctAscList_create_Desc into IH.
+  rewrite fromDistinctAscList_create_eq
+    by (enough (0 < 2^sz)%Z by lia; apply Z.pow_pos_nonneg; lia).
+  unfold fromDistinctAscList_create_f.
+  destruct xs.
+  * intros X HX. apply HX. clear HX.
+    - solve_Bounded.
+    - reflexivity.
+    - left. reflexivity.
+  * repeat replace (#1) with 1%Z by reflexivity.
+    unfold op_zeze__, Eq_Integer___, op_zeze____.
+
+    inversion HSorted. subst.
+    inversion H2. subst. clear H2.
+    inversion H1. subst.
+    destruct p.
+    assert (isUB (safeHd xs) e0 = true). {
+      destruct xs; try reflexivity.
+      inversion H5. subst. unfold safeHd. destruct p. assumption. } 
+    
+    destruct (Z.eqb_spec (2^sz) 1).
+    - intros X HX. apply HX. clear HX.
+      ++ solve_Bounded.
+      ++ rewrite toList_Bin, toList_Tip, app_nil_r. reflexivity.
+      ++ right. rewrite size_Bin. lia.
+    - assert (~ (sz = 0))%Z by (intro; subst; simpl in n; congruence).
+      assert (sz > 0)%Z by lia.
+      replace ((Bits.shiftR (2 ^ sz)%Z 1%Z)) with (2^(sz - 1))%Z.
+      Focus 2.
+        unfold Bits.shiftR, Bits.instance_Bits_Int.
+        rewrite Z.shiftr_div_pow2 by lia.
+        rewrite Z.pow_sub_r by lia.
+        reflexivity.
+      assert (Z.to_nat (sz - 1) < Z.to_nat sz)%nat.
+      { rewrite Z2Nat.inj_sub by lia. 
+        apply Nat.sub_lt.
+        apply Z2Nat.inj_le.
+        lia.
+        lia.
+        lia.
+        replace (Z.to_nat 1) with 1 by reflexivity.
+        lia.
+      }
+      eapply IH.
+      ++ assumption.
+      ++ lia.
+      ++ eassumption.
+      ++ intros l ys HBounded_l Hlist_l Hsize_l.
+         destruct ys.
+         + intros X HX. apply HX. clear HX.
+           ** solve_Bounded.
+           ** assumption.
+           ** left; reflexivity.
+         + simpl in HBounded_l. destruct p.
+           destruct Hsize_l; try congruence.
+           eapply IH; clear IH.
+           ** assumption.
+           ** lia.
+           ** rewrite Hlist_l in H1. 
+              apply StronglySorted_app in H1.
+              destruct H1. 
+              eassumption.
+           ** intros r zs HBounded_r Hlist_r Hsize_r.
+              rewrite Hlist_l in HSorted.
+              assert (isLB (Some lb) e1 = true). {
+                apply StronglySorted_inv in HSorted.
+                destruct HSorted.
+                simpl.
+                rewrite Forall_forall in H10. unfold lt in H10.
+                specialize (H10 (e1, a1)). 
+                apply H10.
+                apply in_or_app. right. left. reflexivity.
+              }
+              rewrite Hlist_r in HSorted.
+              assert (isUB (safeHd zs) e1 = true). {
+                destruct zs; try reflexivity.
+                apply StronglySorted_inv in HSorted.
+                destruct HSorted.
+                apply StronglySorted_app in H10.
+                destruct H10.
+                apply StronglySorted_inv in H12.
+                destruct H12.
+                rewrite Forall_forall in H13. specialize (H13 p). unfold isUB. simpl. destruct p.
+                unfold lt in H13.
+                apply H13.
+                apply in_or_app. right. left. reflexivity.
+              }
+              intros X HX. apply HX. clear HX.
+              -- applyDesc link_Desc.
+              -- erewrite toList_link by eassumption.
+                 rewrite Hlist_l. rewrite Hlist_r.
+                 rewrite <- !app_assoc.  reflexivity.
+              -- destruct Hsize_r; [left; assumption| right].
+                 applyDesc link_Desc.
+                 replace (size l). replace (size r).
+                 rewrite mul_pow_sub in * by lia.
+                 lia.
+Qed.
+
+(*The analogue of [sem] for lists - returns the first value associated with
+a given key, or None if no such key exists. We will use this to
+specify several lemmas in [fromList] rather than List.elem*)
+Fixpoint sem_for_lists (l : list (e * a)) (i : e) :=
+  match l with
+  | nil => None
+  | (x,y) :: t => if i == x then Some y else sem_for_lists t i
+  end.
+
+Lemma sem_list_app: forall i xs ys,
+  sem_for_lists (xs ++ ys) i = sem_for_lists xs i ||| sem_for_lists ys i.
+Proof.
+  intros. generalize dependent ys. induction xs; intros.
+  - simpl. reflexivity.
+  - simpl. destruct a0. destruct (i == e0) eqn : ?. reflexivity.
+    apply IHxs.
+Qed.
+
+Lemma toList_sem'':
+  forall s lb ub, Bounded s lb ub ->
+  forall i, sem s i = sem_for_lists (toList s) i.
+Proof.
+  intros. induction H.
+  - simpl. reflexivity.
+  - simpl. rewrite IHBounded1. rewrite IHBounded2. rewrite toList_Bin.
+    rewrite sem_list_app. rewrite app_comm_cons. rewrite sem_list_app.
+    simpl. unfold SomeIf. rewrite oro_assoc. reflexivity.
+Qed. 
+
+Program Fixpoint fromDistinctAscList_go_Desc
+  sz s xs {measure (length xs)} :
+  (0 <= sz)%Z ->
+  StronglySorted lt xs ->
+  Bounded s None (safeHd xs) ->
+  xs = nil \/ size s = (2*2^sz-1)%Z ->
+  Desc (fromDistinctAscList_go (2^sz)%Z s xs) None None (size s + List.length xs)
+    (fun i => sem s i ||| sem_for_lists xs i) := _. 
+Next Obligation.
+  intros.
+  rename fromDistinctAscList_go_Desc into IH.
+  rewrite fromDistinctAscList_go_eq by (apply Z.pow_pos_nonneg; lia).
+  unfold fromDistinctAscList_go_f.
+  destruct xs.
+  * replace (List.length nil) with 0%Z by reflexivity.
+    rewrite Z.add_0_r.
+    solve_Desc.
+  * repeat replace (#1) with 1%Z by reflexivity.
+    replace ((Bits.shiftL (2 ^ sz)%Z 1))%Z with (2 ^ (1 + sz))%Z.
+    Focus 2.
+      unfold Bits.shiftL, Bits.instance_Bits_Int.
+      rewrite Z.shiftl_mul_pow2 by lia.
+      rewrite Z.pow_add_r by lia.
+      lia. destruct p.
+
+    destruct H2; try congruence.
+    eapply fromDistinctAscList_create_Desc.
+    - lia.
+    - eassumption.
+    - intros.
+      subst.
+      simpl safeHd in *.
+      assert (isUB (safeHd ys) e0 = true). {
+        destruct ys; try reflexivity.
+        apply StronglySorted_inv in H0.
+        destruct H0.
+        rewrite Forall_forall in H4. specialize (H4 p). unfold isUB. destruct p. simpl.
+        unfold lt in H4.
+        apply H4. 
+        apply in_or_app. right. left. reflexivity.
+      }      
+      applyDesc link_Desc.
+      eapply IH.
+      + simpl. rewrite app_length. lia.
+      + lia.
+      + apply StronglySorted_inv in H0.
+        destruct H0.
+        apply StronglySorted_app in H0.
+        destruct H0.
+        assumption.
+      + assumption.
+      + destruct H5; [left; assumption | right].
+        replace (size s1). replace (size s).  replace (size s0).
+        rewrite Z.pow_add_r by lia.
+        lia.
+      + intros.
+        solve_Desc.
+        ** replace (size s2). replace (size s1). replace (size s).
+           rewrite !List.hs_coq_list_length, !Zlength_correct.
+           simpl length.
+           rewrite app_length, Nat2Z.inj_succ, Nat2Z.inj_add.
+           erewrite <- size_spec by eassumption.
+           lia.
+        ** simpl. 
+           setoid_rewrite sem_list_app.
+           setoid_rewrite <- toList_sem''; only 2: eassumption.
+           f_solver.
+Qed.
+
+Lemma fromDistinctAscList_Desc:
+  forall xs,
+  StronglySorted lt xs ->
+  Desc (fromDistinctAscList xs) None None (List.length xs) (fun i => sem_for_lists xs i).
+Proof.
+  intros.
+  unfold fromDistinctAscList.
+  fold fromDistinctAscList_create_f.
+  fold fromDistinctAscList_create.
+  fold fromDistinctAscList_go_f.
+  fold fromDistinctAscList_go.
+  destruct xs.
+  * solve_Desc.
+  * replace (#1) with (2^0)%Z by reflexivity. destruct p.
+    eapply fromDistinctAscList_go_Desc.
+    + lia.
+    + apply StronglySorted_inv in H.
+      destruct H.
+      assumption.
+    + assert (isUB (safeHd xs) e0 = true). {
+        destruct xs; try reflexivity.
+        apply StronglySorted_inv in H.
+        destruct H.
+        rewrite Forall_forall in H0. destruct p. unfold isUB. simpl.
+        unfold lt in H0. specialize (H0 (e1, a1)). 
+        apply H0.
+        left. reflexivity.
+      }
+      solve_Bounded.
+    + right. reflexivity.
+    + intros.
+      rewrite List.hs_coq_list_length, Zlength_cons in *.
+      rewrite size_Bin in *.
+      solve_Desc. simpl. f_solver.
+Qed.
+
+(** ** Verification of [fromDistinctDescList] *)
+
+(** Copy’n’paste from [fromDistinctAscList] *)
+
+Local Definition gt : e * a -> e * a -> Prop
+  := fun x1 x2 => let (e1, a1) := x1 in let (e2, a2) := x2 in (e1 > e2) = true.
+
+Definition fromDistinctDescList_create_f : (Int -> list (e * a) -> (Map e a) * list (e * a)) -> 
+(Int -> list (e * a) -> Map e a * list ( e * a)).
+Proof.
+  let rhs := eval unfold fromDistinctDescList in (@fromDistinctDescList e a) in
+  lazymatch rhs with context [deferredFix2 ?f] => exact f end.
+Defined.
+
+Definition fromDistinctDescList_create : Int -> list (e * a) -> (Map e a) * list (e * a)
+  := deferredFix2 (fromDistinctDescList_create_f).
+
+Lemma fromDistinctDescList_create_eq:
+  forall i xs, (1 <= i)%Z ->
+  fromDistinctDescList_create i xs = fromDistinctDescList_create_f fromDistinctDescList_create i xs.
+Proof.
+  intros.
+  change (uncurry fromDistinctDescList_create (i, xs) = uncurry (fromDistinctDescList_create_f fromDistinctDescList_create) (i, xs)).
+  apply deferredFix_eq_on with
+    (f := fun g => uncurry (fromDistinctDescList_create_f (curry g)))
+    (P := fun p => (1 <= fst p)%Z)
+    (R := fun x y => (1 <= fst x < fst y)%Z).
+  * eapply wf_inverse_image with (R := fun x y => (1 <= x < y)%Z).
+    apply Z.lt_wf with (z := 1%Z).
+  * clear i xs H.
+    intros g h x Px Heq.
+    destruct x as [i xs]. simpl in *.
+    unfold fromDistinctDescList_create_f.
+    destruct_match; try reflexivity.
+    repeat replace (#1) with 1%Z by reflexivity.
+    unfold op_zeze__, Eq_Integer___, op_zeze____.
+    destruct (Z.eqb_spec i 1); try reflexivity.
+    unfold curry.
+    assert (1 < i)%Z by lia.
+    assert (1 <= Z.shiftr i 1)%Z by (apply Z_shiftr_pos; lia).
+    assert (Z.shiftr i 1 < i)%Z by (apply Z_shiftr_lt; lia).
+    repeat expand_pairs. simpl.
+    rewrite Heq by eauto.
+    destruct_match; try reflexivity.
+    rewrite Heq by eauto.
+    reflexivity.
+  * simpl; lia.
+Qed.
+
+(* We need to know that [create] returns no longer list than it receives. *)
+Program Fixpoint fromDistinctDescList_create_preserves_length
+  i xs {measure (Z.to_nat i)} :
+  (1 <= i)%Z ->
+  forall (P : Map e a * list (e * a) -> Prop),
+  ( forall s ys,
+    (length ys <= length xs)%nat ->
+    P (s, ys)
+  ) ->
+  P (fromDistinctDescList_create i xs) := _.
+Next Obligation.
+  intros.
+  rename fromDistinctDescList_create_preserves_length into IH.
+  rewrite fromDistinctDescList_create_eq by assumption.
+  unfold fromDistinctDescList_create_f.
+  destruct xs.
+  * apply H0. reflexivity.
+  * repeat replace (#1) with 1%Z by reflexivity.
+    unfold op_zeze__, Eq_Integer___, op_zeze____.
+    destruct (Z.eqb_spec i 1).
+    + destruct p. apply H0. simpl. lia.
+    + assert (Z.to_nat (Bits.shiftR i #1) < Z.to_nat i)%nat. {
+        apply Z2Nat.inj_lt.
+        apply Z.shiftr_nonneg. lia.
+        lia.
+        apply Z_shiftr_lt; lia.
+      }
+      apply IH.
+      - assumption. 
+      - apply Z_shiftr_pos; lia.
+      - intros.
+        destruct_match.
+        ** apply H0. simpl in *. lia.
+        ** apply IH.
+           -- assumption.
+           -- apply Z_shiftr_pos; lia.
+           -- intros.
+               destruct p0. apply H0. simpl in *. lia.
+Qed.
+
+Definition fromDistinctDescList_go_f : (Int -> Map e a -> list (e * a) -> Map e a) ->
+ (Int -> Map e a -> list (e * a) -> Map e a).
+Proof.
+  let rhs := eval unfold fromDistinctDescList in (@fromDistinctDescList e a) in
+  let rhs := eval fold fromDistinctDescList_create_f in rhs in 
+  let rhs := eval fold fromDistinctDescList_create in rhs in 
+  lazymatch rhs with context [deferredFix3 ?f] => exact f end.
+Defined.
+
+Definition fromDistinctDescList_go : Int -> Map e a -> list (e * a) -> Map e a
+  := deferredFix3 (fromDistinctDescList_go_f).
+
+Lemma fromDistinctDescList_go_eq:
+  forall i s xs, (0 < i)%Z ->
+  fromDistinctDescList_go i s xs = fromDistinctDescList_go_f fromDistinctDescList_go i s xs.
+Proof.
+  intros.
+  change (deferredFix (fun g => uncurry (uncurry (fromDistinctDescList_go_f (curry (curry g))))) (i, s, xs) =
+    uncurry (uncurry (fromDistinctDescList_go_f fromDistinctDescList_go)) (i, s, xs)).
+  rewrite deferredFix_eq_on with
+    (P := fun p => (1 <= fst (fst p))%Z)
+    (R := fun x y => (length (snd x) < length (snd y))%nat); only 1: reflexivity.
+  * apply well_founded_ltof with (f := fun x => length (snd x)).
+  * intros g h p Px Heq.
+    destruct p as [[x y] z].
+    simpl in *.
+    unfold fromDistinctDescList_go_f.
+    destruct_match; try reflexivity.
+    eapply fromDistinctDescList_create_preserves_length; try lia.
+    intros s' ys Hlength. destruct p.
+    apply Heq.
+    + apply Z_shiftl_pos.
+      lia.
+    + simpl. lia.
+  * simpl. lia.
+Qed.
+
+Program Fixpoint fromDistinctDescList_create_Desc
+  sz ub xs x {measure (Z.to_nat sz)} :
+  (0 <= sz)%Z ->
+  StronglySorted (fun x y => gt x y) ((ub, x) :: xs) ->
+  forall (P : (Map e a) * list (e * a) -> Prop),
+  ( forall (s : Map e a) (ys: list (e * a)),
+    Bounded s  (safeHd ys) (Some ub)->
+    xs = rev(toList s) ++ ys ->
+    ys = nil \/ size s = (2*2^sz-1)%Z ->
+    P (s, ys)
+  ) ->
+  P (fromDistinctDescList_create (2^sz)%Z xs) := _.
+Next Obligation.
+  intros ????? Hnonneg HSorted.  
+  rename fromDistinctDescList_create_Desc into IH.
+  rewrite fromDistinctDescList_create_eq
+    by (enough (0 < 2^sz)%Z by lia; apply Z.pow_pos_nonneg; lia).
+  unfold fromDistinctDescList_create_f.
+  destruct xs.
+  * intros X HX. apply HX. clear HX.
+    - solve_Bounded.
+    - reflexivity.
+    - left. reflexivity.
+  * repeat replace (#1) with 1%Z by reflexivity.
+    unfold op_zeze__, Eq_Integer___, op_zeze____.
+
+    inversion HSorted. subst.
+    inversion H2. subst. clear H2.
+    inversion H1. subst.
+    destruct p.
+    assert (isLB (safeHd xs) e0 = true). {
+      destruct xs; try reflexivity.
+      inversion H5. subst. unfold safeHd. destruct p. unfold gt in H6.
+      unfold isLB. order e. } 
+    
+    destruct (Z.eqb_spec (2^sz) 1).
+    - intros X HX. apply HX. clear HX.
+      ++ solve_Bounded. unfold gt in H3. unfold isUB. order e.
+      ++ rewrite toList_Bin, toList_Tip, app_nil_r. reflexivity.
+      ++ right. rewrite size_Bin. lia.
+    - assert (~ (sz = 0))%Z by (intro; subst; simpl in n; congruence).
+      assert (sz > 0)%Z by lia.
+      replace ((Bits.shiftR (2 ^ sz)%Z 1%Z)) with (2^(sz - 1))%Z.
+      Focus 2.
+        unfold Bits.shiftR, Bits.instance_Bits_Int.
+        rewrite Z.shiftr_div_pow2 by lia.
+        rewrite Z.pow_sub_r by lia.
+        reflexivity.
+      assert (Z.to_nat (sz - 1) < Z.to_nat sz)%nat.
+      { rewrite Z2Nat.inj_sub by lia. 
+        apply Nat.sub_lt.
+        apply Z2Nat.inj_le.
+        lia.
+        lia.
+        lia.
+        replace (Z.to_nat 1) with 1 by reflexivity.
+        lia.
+      }
+      eapply IH.
+      ++ assumption.
+      ++ lia.
+      ++ eassumption.
+      ++ intros l ys HBounded_l Hlist_l Hsize_l.
+         destruct ys.
+         + intros X HX. apply HX. clear HX.
+           ** solve_Bounded.
+           ** assumption.
+           ** left; reflexivity.
+         + simpl in HBounded_l. destruct p.
+           destruct Hsize_l; try congruence.
+           eapply IH; clear IH.
+           ** assumption.
+           ** lia.
+           ** rewrite Hlist_l in H1. 
+              apply StronglySorted_app in H1.
+              destruct H1. 
+              eassumption.
+           ** intros r zs HBounded_r Hlist_r Hsize_r.
+              rewrite Hlist_l in HSorted.
+              assert (isUB (Some ub) e1 = true). {
+                apply StronglySorted_inv in HSorted.
+                destruct HSorted.
+                simpl.
+                rewrite Forall_forall in H10. unfold gt in H10.
+                specialize (H10 (e1, a1)). 
+                assert (e1 < ub = true <-> ub > e1 = true) by (order e). rewrite H11.
+                apply H10.
+                apply in_or_app. right. left. reflexivity.
+              }
+              rewrite Hlist_r in HSorted.
+              assert (isLB (safeHd zs) e1 = true). {
+                destruct zs; try reflexivity.
+                apply StronglySorted_inv in HSorted.
+                destruct HSorted.
+                apply StronglySorted_app in H10.
+                destruct H10.
+                apply StronglySorted_inv in H12.
+                destruct H12.
+                rewrite Forall_forall in H13. specialize (H13 p). unfold isLB. simpl. destruct p.
+                unfold gt in H13. assert (e2 < e1 = true <-> e1 > e2 = true) by (order e).
+                rewrite H14.
+                apply H13.
+                apply in_or_app. right. left. reflexivity.
+              }
+              intros X HX. apply HX. clear HX.
+              -- applyDesc link_Desc.
+              -- erewrite toList_link by eassumption.
+                 rewrite Hlist_l. rewrite Hlist_r.
+                 rewrite !rev_app_distr; simpl.
+                 rewrite <- !app_assoc.  simpl. reflexivity.
+              -- destruct Hsize_r; [left; assumption| right].
+                 applyDesc link_Desc.
+                 replace (size l). replace (size r).
+                 rewrite mul_pow_sub in * by lia.
+                 lia.
+Qed.
+
+(*If we look for an element in a map's list, it is the same as looking in the reverse of that list.
+This is euivalent to saying that the first key, value pair that matches a given key is the same
+as the last pair*)
+Lemma sem_list_rev:
+  forall m lb ub x,
+  Bounded m lb ub ->
+  sem_for_lists (toList m) x = sem_for_lists (rev (toList m)) x.
+Proof.
+  intros. generalize dependent x. induction H; intros.
+  - simpl. reflexivity.
+  - rewrite toList_Bin. rewrite rev_app_distr.
+ simpl. rewrite <- app_assoc. simpl.
+    rewrite sem_list_app. rewrite sem_list_app. rewrite <- IHBounded2.
+    assert (forall {a} (x : a) l, x :: l = (x :: nil) ++ l). { intros.
+    simpl. reflexivity. } rewrite H5. rewrite sem_list_app.
+    rewrite (H5 _ _ (rev (toList s1))). rewrite sem_list_app.
+    rewrite <- IHBounded1. repeat(erewrite <- toList_sem'').
+    destruct (sem s1 x0) eqn : ?. simpl.
+    assert (sem s2 x0 = None). { eapply sem_outside_below. apply H0. solve_Bounds. }
+    rewrite H6. simpl. assert (x0 == x = false) by solve_Bounds. rewrite H7; reflexivity.
+    simpl. destruct (x0 == x) eqn : ?. assert (sem s2 x0 = None). { eapply sem_outside_below.
+    apply H0. solve_Bounds. } rewrite H6. reflexivity. simpl. rewrite oro_None_r. reflexivity.
+    apply H0. apply H.
+Qed.
+
+Program Fixpoint fromDistinctDescList_go_Desc
+  sz s xs {measure (length xs)} :
+  (0 <= sz)%Z ->
+  StronglySorted (fun x y => gt x y) xs ->
+  Bounded s (safeHd xs) None  ->
+  xs = nil \/ size s = (2*2^sz-1)%Z ->
+  Desc (fromDistinctDescList_go (2^sz)%Z s xs) None None (size s + List.length xs)
+    (fun i => sem s i ||| sem_for_lists xs i) := _. 
+Next Obligation.
+  intros.
+  rename fromDistinctDescList_go_Desc into IH.
+  rewrite fromDistinctDescList_go_eq by (apply Z.pow_pos_nonneg; lia).
+  unfold fromDistinctDescList_go_f.
+  destruct xs.
+  * replace (List.length nil) with 0%Z by reflexivity.
+    rewrite Z.add_0_r.
+    solve_Desc.
+  * repeat replace (#1) with 1%Z by reflexivity.
+    replace ((Bits.shiftL (2 ^ sz)%Z 1))%Z with (2 ^ (1 + sz))%Z.
+    Focus 2.
+      unfold Bits.shiftL, Bits.instance_Bits_Int.
+      rewrite Z.shiftl_mul_pow2 by lia.
+      rewrite Z.pow_add_r by lia.
+      lia. destruct p.
+
+    destruct H2; try congruence.
+    eapply fromDistinctDescList_create_Desc.
+    - lia.
+    - eassumption.
+    - intros.
+      subst.
+      simpl safeHd in *.
+      assert (isLB (safeHd ys) e0 = true). {
+        destruct ys; try reflexivity.
+        apply StronglySorted_inv in H0.
+        destruct H0.
+        rewrite Forall_forall in H4. specialize (H4 p). unfold isLB. destruct p. simpl.
+        unfold gt in H4. assert (e1 < e0 = true <->e0 > e1 = true) by (order e). rewrite H6.
+        apply H4. 
+        apply in_or_app. right. left. reflexivity.
+      }      
+      applyDesc link_Desc.
+      eapply IH.
+      + simpl. rewrite app_length. lia.
+      + lia.
+      + apply StronglySorted_inv in H0.
+        destruct H0.
+        apply StronglySorted_app in H0.
+        destruct H0.
+        assumption.
+      + assumption.
+      + destruct H5; [left; assumption | right].
+        replace (size s1). replace (size s).  replace (size s0).
+        rewrite Z.pow_add_r by lia.
+        lia.
+      + intros.
+        solve_Desc.
+        ** replace (size s2). replace (size s1). replace (size s).
+           rewrite !List.hs_coq_list_length, !Zlength_correct.
+           simpl length.
+           rewrite app_length, Nat2Z.inj_succ, Nat2Z.inj_add, rev_length.
+           erewrite <- size_spec by eassumption.
+           lia.
+        ** simpl. setoid_rewrite sem_list_app. 
+            assert (forall i, sem_for_lists (rev (toList s0)) i = sem_for_lists (toList s0) i).
+            setoid_rewrite (sem_list_rev s0 (safeHd ys) (Some e0) _ H3). intros. reflexivity. 
+            setoid_rewrite H9.
+            setoid_rewrite <- toList_sem''; only 2: eassumption.
+            f_solver.
+Qed.
+
+
+
+Lemma fromDistinctDescList_Desc:
+  forall xs,
+  StronglySorted (fun x y => gt x y) xs ->
+  Desc (fromDistinctDescList xs) None None (List.length xs) (fun i => sem_for_lists xs i).
+Proof.
+  intros.
+  unfold fromDistinctDescList.
+  fold fromDistinctDescList_create_f.
+  fold fromDistinctDescList_create.
+  fold fromDistinctDescList_go_f.
+  fold fromDistinctDescList_go.
+  destruct xs.
+  * solve_Desc.
+  * replace (#1) with (2^0)%Z by reflexivity. destruct p.
+    eapply fromDistinctDescList_go_Desc.
+    + lia.
+    + apply StronglySorted_inv in H.
+      destruct H.
+      assumption.
+    + assert (isLB (safeHd xs) e0 = true). {
+        destruct xs; try reflexivity.
+        apply StronglySorted_inv in H.
+        destruct H.
+        rewrite Forall_forall in H0. destruct p. unfold isLB. simpl.
+        unfold gt in H0. specialize (H0 (e1, a1)). 
+        assert (e1 < e0 = true <-> e0 > e1 = true) by (order e). rewrite H1.
+        apply H0.
+        left. reflexivity.
+      }
+      solve_Bounded.
+    + right. reflexivity.
+    + intros.
+      rewrite List.hs_coq_list_length, Zlength_cons in *.
+      rewrite size_Bin in *.
+      solve_Desc. simpl. f_solver.
+Qed.
+
+(** ** Verification of [combineEq] *)
+
+(*Since [combineEq'] and [combineEq] are defined inside [fromAscList] (unlike in Data.Set), we define them here
+and then prove equivalence*)
+
+Fixpoint combineEq' {e} {a} `{EqLaws e} (x : e * a) (l : list (e * a) ) :=
+  match x, l with
+  |z, nil => z :: nil
+  |(a, b), (c, d) :: t => if a == c then combineEq' (c, d) t else (a,b) :: combineEq' (c,d) t
+  end.
+
+(*The combineEq' from Data.Map (defined here to make combineEq'_equiv nicer*)
+Definition old_combineEq' :=(fix combineEq' (arg_0__ : e * a) (arg_1__ : list (e * a)) {struct arg_1__} : list (e * a) :=
+   let (kz, _) := arg_0__ in
+   match arg_1__ with
+   | nil => arg_0__ :: nil
+   | (kx, xx) as x :: xs' => if _GHC.Base.==_ kx kz then combineEq' (kx, xx) xs' else arg_0__ :: combineEq' x xs'
+   end).
+
+Definition combineEq {e} {a} `{EqLaws e} (l : list (e * a)) :=
+  match l with
+  | nil => nil
+  | x :: nil => x :: nil
+  | x :: t => combineEq' x t
+  end.
+
+Lemma combineEq'_equiv:
+  forall l x, combineEq' x l = old_combineEq' x l.
+Proof.
+  intros. revert x. induction l; intros.
+  - simpl. destruct x. reflexivity.
+  - simpl. destruct x. destruct a0. destruct (e0 == e1) eqn : ?.
+    assert (e1 == e0 = true) by (order e). rewrite H. apply IHl.
+    assert (e1 == e0 = false) by (order e). rewrite H. rewrite IHl.
+    reflexivity.
+Qed.
+
+
+Definition fromAscList' (l : list (e * a)) :=
+  fromDistinctAscList (combineEq l).
+
+
+Lemma fromAscList_equiv: forall (l : list (e * a)),
+  fromAscList' l = fromAscList l.
+Proof.
+  intros l. unfold fromAscList', fromAscList. destruct l.
+  - simpl. reflexivity.
+  -  unfold combineEq. rewrite combineEq'_equiv. unfold old_combineEq'.
+     reflexivity.
+Qed.
+
+Definition fromDescList' (l : list (e * a)) :=
+  fromDistinctDescList (combineEq l).
+
+Lemma fromDescList_equiv: forall (l : list (e * a)),
+  fromDescList' l = fromDescList l.
+Proof.
+  intros l. unfold fromDescList', fromDescList. destruct l.
+  - simpl. reflexivity.
+  -  unfold combineEq. rewrite combineEq'_equiv. unfold old_combineEq'.
+     reflexivity.
+Qed.
+
+Definition combineEqGo : (e * a) -> list (e * a) -> list (e * a).
+Proof.
+  intros.
+ apply (@combineEq' e a HEq HEqLaws). apply X.  apply X0.
+Defined.
+
+(* Too much duplication here *)
+
+(*See if a key is a (key, value) list*)
+Fixpoint key_elem (l : list (e * a)) i :=
+  match l with
+  | nil => false
+  | (x, y) :: t => (x == i) || key_elem t i
+  end.
+
+(*This finds the last value associated with a key in a list*)
+Fixpoint last_value (l : list (e * a)) i:=
+  match l with
+  | nil => None
+  | (x, y) :: t => if (x == i) then match last_value t i with
+                               | None => Some y
+                               | Some z => Some z
+                               end else last_value t i
+  end. 
+
+(*This proves that the last_value does in fact find the last value, since it finds
+the first value in the reversed list. It also justifies using either
+[sem_for_lists (rev l)] or [last_value l] based on which is more convienent. For 
+[combineEq] and [fromDescList] (and similar), I use [last_value l], and in
+from_list, I use [sem_for_lists (rev l)]*)
+Lemma last_sem_equiv: forall l x,
+  sem_for_lists (rev l) x = last_value l x.
+Proof.
+  intros. revert x; induction l; intros.
+  - simpl. reflexivity.
+  - simpl. destruct a0. rewrite sem_list_app. rewrite IHl.
+    simpl. destruct (e0 == x) eqn : ?. assert (x == e0 = true) by (order e).
+    rewrite H. destruct (last_value l x) eqn : ?. simpl. reflexivity. simpl. reflexivity.
+    assert (x == e0 = false) by (order e). rewrite H. rewrite oro_None_r. reflexivity.
+Qed. 
+
+(*An element has a last occurrence iff it is in the list*)
+Lemma last_iff_elem: forall l i,
+  (exists v, last_value l i = Some v) <-> key_elem l i = true.
+Proof.
+  intros. revert  i. induction l; split; intros.
+  - simpl in H. inversion H. inversion H0.
+  - simpl in H. inversion H. 
+  - simpl. destruct a0.  simpl in H. destruct (e0 == i) eqn : ?.
+    simpl. reflexivity. simpl. eapply IHl. apply H.
+  - simpl. destruct a0. simpl in H. destruct (e0  == i) eqn : ?.
+    destruct (last_value l i) eqn : ?. exists a1. reflexivity.
+    exists a0. reflexivity. simpl in H. apply IHl. apply H.
+Qed.
+
+Local Definition le : e * a -> e * a -> Prop
+  := fun x1 x2 => let (e1, a1) := x1 in let (e2, a2) := x2 in (e1 <= e2) = true.
+  
+Lemma Forall_le_elem:
+  forall x x0 xs,
+  Forall (fun y => le (x, x0) y) xs <-> (forall i, key_elem xs i = true -> x <= i = true).
+Proof.
+  intros.
+  induction xs.
+  * split; intro H.
+    - intros i Hi; simpl in Hi; congruence.
+    - constructor.
+  * split; intro H.
+    - inversion H; subst; clear H.
+      rewrite IHxs in H3; clear IHxs.
+      intros i Hi; simpl in Hi. destruct a0. 
+      rewrite orb_true_iff in Hi. destruct Hi.
+      + unfold le in *.  order e.
+      + apply H3; assumption.
+    - constructor.
+      + unfold le. destruct a0. apply H. simpl. rewrite Eq_Reflexive. simpl. reflexivity.
+      + rewrite IHxs; clear IHxs.
+        intros i Hi. apply H. simpl. rewrite Hi. destruct a0.  apply orb_true_r.
+Qed.
+
+Lemma Forall_le_last:
+  forall x x0 xs,
+  Forall (fun y => le (x, x0) y) xs <-> (forall i v, last_value xs i = Some v -> x <= i = true).
+Proof.
+  intros.
+  rewrite Forall_le_elem. split; intros.
+  - apply H. apply last_iff_elem. exists v. assumption.
+  - apply last_iff_elem in H0. destruct H0. apply H in H0. assumption.
+Qed. 
+
+
+Local Definition ge : e * a -> e * a -> Prop
+  := fun x1 x2 => let (e1, a1) := x1 in let (e2, a2) := x2 in (e1 >= e2) = true.
+
+Lemma Forall_ge_elem:
+  forall x x0 xs,
+  Forall (fun y => ge (x, x0) y) xs <-> (forall i, key_elem xs i = true -> x >= i = true).
+Proof.
+  intros.
+  induction xs.
+  * split; intro H.
+    - intros i Hi; simpl in Hi; congruence.
+    - constructor.
+  * split; intro H.
+    - inversion H; subst; clear H.
+      rewrite IHxs in H3; clear IHxs.
+      intros i Hi; simpl in Hi. destruct a0. 
+      rewrite orb_true_iff in Hi. destruct Hi.
+      + unfold ge in *.  order e.
+      + apply H3; assumption.
+    - constructor.
+      + unfold ge. destruct a0. apply H. simpl. rewrite Eq_Reflexive. simpl. reflexivity.
+      + rewrite IHxs; clear IHxs.
+        intros i Hi. apply H. simpl. rewrite Hi. destruct a0.  apply orb_true_r.
+Qed.
+
+Lemma Forall_ge_last:
+  forall x x0 xs,
+  Forall (fun y => ge (x, x0) y) xs <-> (forall i v, last_value xs i = Some v -> x >= i = true).
+Proof.
+  intros.
+  rewrite Forall_ge_elem. split; intros.
+  - apply H. apply last_iff_elem. exists v. assumption.
+  - apply last_iff_elem in H0. destruct H0. apply H in H0. assumption.
+Qed. 
+
+Lemma Forall_lt_elem:
+  forall x x0 xs,
+  Forall (fun y => lt (x, x0) y) xs <-> (forall i, key_elem xs i = true -> x < i = true).
+Proof.
+  intros.
+  induction xs.
+  * split; intro H.
+    - intros i Hi; simpl in Hi; congruence.
+    - constructor.
+  * split; intro H.
+    - inversion H; subst; clear H.
+      rewrite IHxs in H3; clear IHxs.
+      intros i Hi; simpl in Hi. destruct a0. 
+      rewrite orb_true_iff in Hi. destruct Hi.
+      + unfold lt in *.  order e.
+      + apply H3; assumption.
+    - constructor.
+      + unfold lt. destruct a0. apply H. simpl. rewrite Eq_Reflexive. simpl. reflexivity.
+      + rewrite IHxs; clear IHxs.
+        intros i Hi. apply H. simpl. rewrite Hi. destruct a0.  apply orb_true_r.
+Qed.
+
+Lemma Forall_lt_last:
+  forall x x0 xs,
+  Forall (fun y => lt (x, x0) y) xs <-> (forall i v, last_value xs i = Some v -> x < i = true).
+Proof.
+  intros.
+  rewrite Forall_lt_elem. split; intros.
+  - apply H. apply last_iff_elem. exists v. assumption.
+  - apply last_iff_elem in H0. destruct H0. apply H in H0. assumption.
+Qed. 
+
+
+Lemma Forall_gt_elem:
+  forall x x0 xs,
+  Forall (fun y => gt (x, x0) y) xs <-> (forall i, key_elem xs i = true -> x > i = true).
+Proof.
+  intros.
+  induction xs.
+  * split; intro H.
+    - intros i Hi; simpl in Hi; congruence.
+    - constructor.
+  * split; intro H.
+    - inversion H; subst; clear H.
+      rewrite IHxs in H3; clear IHxs.
+      intros i Hi; simpl in Hi. destruct a0. 
+      rewrite orb_true_iff in Hi. destruct Hi.
+      + unfold gt in *.  order e.
+      + apply H3; assumption.
+    - constructor.
+      + unfold gt. destruct a0. apply H. simpl. rewrite Eq_Reflexive. simpl. reflexivity.
+      + rewrite IHxs; clear IHxs.
+        intros i Hi. apply H. simpl. rewrite Hi. destruct a0.  apply orb_true_r.
+Qed.
+
+Lemma Forall_gt_last:
+  forall x x0 xs,
+  Forall (fun y => gt (x, x0) y) xs <-> (forall i v, last_value xs i = Some v -> x > i = true).
+Proof.
+  intros.
+  rewrite Forall_gt_elem. split; intros.
+  - apply H. apply last_iff_elem. exists v. assumption.
+  - apply last_iff_elem in H0. destruct H0. apply H in H0. assumption.
+Qed. 
+
+
+(*Note: This is significatly different than SetProofs. It is not enough that the keys are preserved,
+we must show that each key is matched with its last value in the list*)
+Lemma combineEqGo_spec:
+  forall x xs,
+  StronglySorted (fun x y => le x y) (x :: xs) ->
+  forall P : list (e * a) -> Prop,
+  (forall (ys: list (e * a)),
+     StronglySorted (fun x y => lt x y) ys ->
+     (forall i, last_value ys i = last_value (x :: xs) i) ->
+     P ys) ->
+  P (combineEqGo x xs).
+Proof.
+  intros x xs Hsorted.
+  inversion Hsorted; subst; clear Hsorted.
+  revert x H2.
+  induction H1; intros x Hlt.
+  * intros X HX; apply HX; clear X HX.
+    + unfold lt. unfold le in Hlt. unfold combineEqGo. simpl. destruct x.
+      constructor; constructor.
+    + intro. unfold combineEqGo. simpl. destruct x. simpl. reflexivity.
+  * inversion Hlt; subst; clear Hlt.  
+    simpl. unfold combineEqGo in *. simpl in *. destruct a0. destruct x.
+    destruct_match.
+    + eapply IHStronglySorted; only 1: assumption; intros ys Hsortedys Hiys.
+      intros X HX; apply HX; clear X HX.
+      - assumption.
+      - intro i. rewrite Hiys. simpl. 
+        destruct (e0 == i) eqn:?, (e1 == i) eqn:?. destruct (last_value l i) eqn : ?.
+        reflexivity. reflexivity. reflexivity. order e. reflexivity.
+    + assert (Hlt : e1 < e0 = true) by (unfold le in H3; order e). clear H3 Heq.
+      eapply IHStronglySorted; only 1: assumption; intros ys Hsortedys Hiys.
+      intros X HX; apply HX; clear X HX.
+      - constructor.
+        ** eapply StronglySorted_R_ext; only 2: apply Hsortedys.
+           intros. simpl. order e.
+        ** apply Forall_lt_last.
+           rewrite Forall_le_last in H.
+           intros i v Hi. rewrite Hiys in Hi.  simpl in Hi. unfold lt.
+           destruct (e0 == i) eqn : ?. order e. apply H in Hi. unfold le in Hi. order e.
+      - intro i. simpl. rewrite Hiys. simpl. reflexivity.
+Qed.
+
+Lemma combineEqGo_spec2:
+  forall x xs,
+  StronglySorted (fun x y => ge x y) (x :: xs) ->
+  forall P : list (e * a) -> Prop,
+  (forall (ys: list (e * a)),
+     StronglySorted (fun x y => gt x y) ys ->
+     (forall i, last_value ys i = last_value (x :: xs) i) ->
+     P ys) ->
+  P (combineEqGo x xs).
+Proof.
+  intros x xs Hsorted.
+  inversion Hsorted; subst; clear Hsorted.
+  revert x H2.
+  induction H1; intros x Hlt.
+  * intros X HX; apply HX; clear X HX.
+    + unfold lt. unfold ge in Hlt. unfold combineEqGo. simpl. destruct x.
+      constructor; constructor.
+    + intro. unfold combineEqGo. simpl. destruct x.  simpl. reflexivity.
+  * inversion Hlt; subst; clear Hlt.  
+    simpl. unfold combineEqGo in *. simpl in *. destruct a0. destruct x.
+    destruct_match.
+    + eapply IHStronglySorted; only 1: assumption; intros ys Hsortedys Hiys.
+      intros X HX; apply HX; clear X HX.
+      - assumption.
+      - intro i. rewrite Hiys. simpl. 
+        destruct (e0 == i) eqn:?, (e1 == i) eqn:?. destruct (last_value l i) eqn : ?.
+        reflexivity. reflexivity. reflexivity. order e. reflexivity.
+    + assert (Hlt : e1 > e0 = true) by (unfold ge in H3; order e). clear H3 Heq.
+      eapply IHStronglySorted; only 1: assumption; intros ys Hsortedys Hiys.
+      intros X HX; apply HX; clear X HX.
+      - constructor.
+        ** eapply StronglySorted_R_ext; only 2: apply Hsortedys.
+           intros. simpl. order e.
+        ** apply Forall_gt_last.
+           rewrite Forall_ge_last in H.
+           intros i v Hi. rewrite Hiys in Hi.  simpl in Hi. unfold lt.
+           destruct (e0 == i) eqn : ?. order e. apply H in Hi. unfold ge in Hi. order e.
+      - intro i. simpl. rewrite Hiys. simpl. reflexivity.
+Qed.
+
+Lemma combineEq_spec:
+  forall xs,
+  StronglySorted (fun x y => le x  y) xs ->
+  forall P : list (e * a) -> Prop,
+  (forall ys,
+     StronglySorted (fun x y => lt x y) ys ->
+     (forall i, last_value ys i = last_value xs i) ->
+     P ys) ->
+  P (combineEq xs).
+Proof.
+  intros xs Hsorted.
+  inversion Hsorted.
+  * intros X HX. apply HX. clear X HX.
+    - constructor.
+    - intro. reflexivity.
+  * rewrite <- H1 in Hsorted. clear xs H0 H1.
+    assert (combineEq (a0 :: l) = combineEqGo a0 l). {
+    unfold combineEqGo. simpl. destruct l. simpl. destruct a0. reflexivity.
+    reflexivity. } rewrite H0.
+    apply combineEqGo_spec. assumption.
+Qed.
+
+Lemma combineEq_spec2:
+  forall xs,
+  StronglySorted (fun x y => ge x  y) xs ->
+  forall P : list (e * a) -> Prop,
+  (forall ys,
+     StronglySorted (fun x y => gt x y) ys ->
+     (forall i, last_value ys i = last_value xs i) ->
+     P ys) ->
+  P (combineEq xs).
+Proof.
+  intros xs Hsorted.
+  inversion Hsorted.
+  * intros X HX. apply HX. clear X HX.
+    - constructor.
+    - intro. reflexivity.
+  * rewrite <- H1 in Hsorted. clear xs H0 H1.
+    assert (combineEq (a0 :: l) = combineEqGo a0 l). {
+    unfold combineEqGo. simpl. destruct l. simpl. destruct a0. reflexivity.
+    reflexivity. } rewrite H0.
+    apply combineEqGo_spec2. assumption.
+Qed.
+
+
+(** ** Verification of [fromAscList] *)
+
+(*See whether a key, value pair is in a list, comparing the keys with Haskell equality
+and the values with Coq equality. This will be used in place of List.In in the following
+analogues of [Forall_forall]*)
+Fixpoint weak_In (l : list (e * a)) (x : e * a) :=
+  match l with
+  | nil => False
+  | (a,b) :: t => let (x0, y0) := x in (a == x0 = true) /\ b = y0 \/ weak_In t x
+  end.
+
+Lemma Forall_forall_lt: 
+  forall  (l : list (e * a)) t, Forall (lt t) l <-> (forall x, weak_In l x -> lt t x).
+Proof.
+  intros. split; intros; induction l; intros.
+  - simpl in H0. destruct H0.
+  - simpl in H0. destruct a0. destruct x. destruct H0. inversion H; subst.
+    destruct H0. subst. destruct t. unfold lt in *. order e.
+  - apply IHl. inversion H; subst. assumption. apply H0.
+  - apply Forall_nil.
+  - apply Forall_cons. simpl in H. destruct a0. apply H. left.
+    split. apply Eq_Reflexive. reflexivity. simpl in H.
+    destruct a0. apply IHl. intros. apply H. destruct x. right. assumption.
+Qed.
+
+Lemma Forall_forall_gt: 
+  forall  (l : list (e * a)) t, Forall (gt t) l <-> (forall x, weak_In l x -> gt t x).
+Proof.
+  intros. split; intros; induction l; intros.
+  - simpl in H0. destruct H0.
+  - simpl in H0. destruct a0. destruct x. destruct H0. inversion H; subst.
+    destruct H0. subst. destruct t. unfold gt in *. order e.
+  - apply IHl. inversion H; subst. assumption. apply H0.
+  - apply Forall_nil.
+  - apply Forall_cons. simpl in H. destruct a0. apply H. left.
+    split. apply Eq_Reflexive. reflexivity. simpl in H.
+    destruct a0. apply IHl. intros. apply H. destruct x. right. assumption.
+Qed.
+
+Lemma strongly_sorted_in_sem_lt: forall l x v,
+  StronglySorted lt l ->
+  sem_for_lists l x = Some v <-> weak_In l (x,v).
+Proof.
+  intros; revert x v; induction l; intros; split; intros.
+  - inversion H0.
+  - destruct H0.
+  - simpl. simpl in H0. destruct a0. destruct (x == e0) eqn : ?.
+    left. split. order e. inversion H0; subst; reflexivity.
+    right. apply IHl. inversion H; subst; assumption. apply H0.
+  - simpl in H0. simpl. destruct a0.
+    destruct H0. destruct H0. subst. assert (x == e0 = true) by (order e).
+    rewrite H1. reflexivity. inversion H; subst.
+    rewrite Forall_forall_lt in H4. assert (A:=H0). apply H4 in H0. unfold lt in H0.
+    assert (x == e0 = false) by (order e). rewrite H1. apply IHl. apply H3. apply A.
+Qed.
+
+Lemma strongly_sorted_in_sem_gt: forall l x v,
+  StronglySorted gt l ->
+  sem_for_lists l x = Some v <-> weak_In l (x,v).
+Proof.
+  intros; revert x v; induction l; intros; split; intros.
+  - inversion H0.
+  - destruct H0.
+  - simpl. simpl in H0. destruct a0. destruct (x == e0) eqn : ?.
+    left. split. order e. inversion H0; subst; reflexivity.
+    right. apply IHl. inversion H; subst; assumption. apply H0.
+  - simpl in H0. simpl. destruct a0.
+    destruct H0. destruct H0. subst. assert (x == e0 = true) by (order e).
+    rewrite H1. reflexivity. inversion H; subst.
+    rewrite Forall_forall_gt in H4. assert (A:=H0). apply H4 in H0. unfold gt in H0.
+    assert (x == e0 = false) by (order e). rewrite H1. apply IHl. apply H3. apply A.
+Qed.
+
+Lemma strongly_sorted_last_lt:
+  forall l x,
+  StronglySorted lt l ->
+  last_value l x = sem_for_lists l x.
+Proof.
+  intros. revert x. induction H; intros.
+  - simpl. reflexivity.
+  - simpl. destruct a0. destruct (x == e0) eqn : ?.
+    rewrite Forall_forall_lt in H0.
+    rewrite IHStronglySorted.
+    destruct (sem_for_lists l x) eqn : ?. 
+    + rewrite strongly_sorted_in_sem_lt in Heqo. apply H0 in Heqo.
+      unfold lt in Heqo. order e. apply H. destruct (e0 == x) eqn : ?. reflexivity.
+    order e. assert (e0 == x = false) by (order e). rewrite H1. apply IHStronglySorted.
+Qed.
+
+Lemma strongly_sorted_last_gt:
+  forall l x,
+  StronglySorted gt l ->
+  last_value l x = sem_for_lists l x.
+Proof.
+  intros. revert x. induction H; intros.
+  - simpl. reflexivity.
+  - simpl. destruct a0. destruct (x == e0) eqn : ?.
+    rewrite Forall_forall_gt in H0.
+    rewrite IHStronglySorted.
+    destruct (sem_for_lists l x) eqn : ?. 
+    + rewrite strongly_sorted_in_sem_gt in Heqo. apply H0 in Heqo.
+      unfold gt in Heqo. order e. apply H. destruct (e0 == x) eqn : ?. reflexivity.
+    order e. assert (e0 == x = false) by (order e). rewrite H1. apply IHStronglySorted.
+Qed.
+
+
+Lemma fromAscList_Desc:
+  forall xs,
+  StronglySorted (fun x y => le x y) xs ->
+  Desc' (fromAscList xs) None None (fun i => last_value xs i).
+Proof.
+  intros. rewrite <- fromAscList_equiv. unfold fromAscList'.
+  eapply combineEq_spec; only 1: assumption; intros ys HSorted Helem.
+  apply fromDistinctAscList_Desc; only 1: assumption.
+  intros s HB Hsz Hf.
+  solve_Desc. intros. rewrite <- Helem. rewrite strongly_sorted_last_lt.
+  apply Hf. apply HSorted.
+Qed.
+
+(** ** Verification of [fromDescList] *)
+
+Lemma fromDescList_Desc:
+  forall xs,
+  StronglySorted (fun x y => ge x y) xs ->
+  Desc' (fromDescList xs) None None (fun i => last_value xs i).
+Proof.
+  intros. rewrite <- fromDescList_equiv. unfold fromDescList'.
+  unfold fromDescList.
+  eapply combineEq_spec2;  only 1: assumption; intros ys HSorted Helem.
+  apply fromDistinctDescList_Desc; only 1: assumption.
+  intros s HB Hsz Hf.
+  solve_Desc. intros. rewrite <- Helem. rewrite strongly_sorted_last_gt.
+  apply Hf. apply HSorted.
+Qed.
+
+(** ** Verification of [fromList] *)
+
+(** The verification of [fromList] should be similar to that of [fromDistinctAscList], only
+that the condition is checked and -- if it fails -- we resort to a backup implementation. *)
+
+(* The following definitions are copied from the local definitions of [fromList]; 
+   my ltac foo failed to do that automatic.
+*)
+
+Definition fromList' :=
+          fun (t0: Map e a) (xs: list (e * a)) =>
+            let ins :=
+              fun arg_2__ arg_3__ =>
+                match arg_2__, arg_3__ with
+                | t, pair k x => insert k x t
+                end in
+            Data.Foldable.foldl' ins t0 xs.
+
+Definition not_ordered :=
+          fun (arg_7__ : e) (arg_8__: list (e * a)) =>
+            match arg_7__, arg_8__ with
+            | _, nil => false
+            | kx, cons (pair ky _) _ => kx GHC.Base.>= ky
+            end .
+
+Definition fromList_create_f : (Int -> list (e * a) -> Map e a * list (e * a) * list (e * a)) -> 
+(Int -> list (e * a) -> Map e a * list (e * a)  * list (e * a))
+  := (fun create arg_11__ arg_12__ =>
+      match arg_11__, arg_12__ with
+      | _, nil => pair (pair Tip nil) nil
+      | s, (cons xp xss as xs) =>
+       if s GHC.Base.== #1 : bool
+       then let 'pair kx x := xp in
+         if not_ordered kx xss : bool
+         then pair (pair (Bin #1 kx x Tip Tip) nil) xss else
+         pair (pair (Bin #1 kx x Tip Tip) xss) nil else
+         match create (Data.Bits.shiftR s #1) xs with
+         | (pair (pair _ nil) _ as res) => res
+         | pair (pair l (cons (pair ky y) nil)) zs =>
+              pair (pair (insertMax ky y l) nil) zs
+         | pair (pair l (cons (pair ky y) yss as ys)) _ =>
+             if not_ordered ky yss : bool then pair (pair l nil) ys else
+             let 'pair (pair r zs) ws := create (Data.Bits.shiftR s #1) yss in
+                       pair (pair (link ky y l r) zs) ws
+         end
+       end).
+
+Definition fromList_create : Int -> list (e * a) -> Map e a * list (e * a) * list (e * a)
+  := deferredFix2 (fromList_create_f).
+
+Definition fromList_go_f :=
+  (fun (go: Int -> Map e a -> list (e * a) -> Map e a) (arg_28__ : Int)
+   (arg_29__ : Map e a) (arg_30__: list (e * a)) =>
+    match arg_28__, arg_29__, arg_30__ with
+    | _, t, nil => t
+    | _, t, cons (pair kx x) nil => insertMax kx x t
+    | s, l, (cons (pair kx x) xss as xs) =>
+          if not_ordered kx xss : bool then fromList' l xs else
+          match fromList_create s xss with
+          | pair (pair r ys) nil => go (Data.Bits.shiftL s #1) (link kx x l r) ys
+          | pair (pair r _) ys => fromList' (link kx x l r) ys
+          end
+   end).
+
+Definition fromList_go := deferredFix3 (fromList_go_f).
+
+(** zeta-reduces exactly one (the outermost) [let] *)
+Ltac zeta_one :=
+  lazymatch goal with |- context A [let x := ?rhs in @?body x] =>
+     let e' := eval cbv beta in (body rhs) in
+     let e'' := context A [e'] in
+     change e''
+  end.
+
+(* Identical to [fromDistinctAscList_create_eq] *)
+Lemma fromList_create_eq:
+  forall i xs, (1 <= i)%Z ->
+  fromList_create i xs = fromList_create_f fromList_create i xs.
+Proof.
+  intros.
+  change (uncurry fromList_create (i, xs) = uncurry (fromList_create_f fromList_create) (i, xs)).
+  apply deferredFix_eq_on with
+    (f := fun g => uncurry (fromList_create_f (curry g)))
+    (P := fun p => (1 <= fst p)%Z)
+    (R := fun x y => (1 <= fst x < fst y)%Z).
+  * eapply wf_inverse_image with (R := fun x y => (1 <= x < y)%Z).
+    apply Z.lt_wf with (z := 1%Z).
+  * clear i xs H.
+    intros g h x Px Heq.
+    destruct x as [i xs]. simpl in *.
+    unfold fromList_create_f.
+    destruct_match; try reflexivity.
+    repeat replace (#1) with 1%Z by reflexivity.
+    unfold op_zeze__, Eq_Integer___, op_zeze____.
+    destruct (Z.eqb_spec i 1); try reflexivity.
+    unfold curry.
+    assert (1 < i)%Z by lia.
+    assert (1 <= Z.shiftr i 1)%Z by (apply Z_shiftr_pos; lia).
+    assert (Z.shiftr i 1 < i)%Z by (apply Z_shiftr_lt; lia).
+    repeat expand_pairs. simpl.
+    rewrite Heq by eauto.
+    destruct_match; try reflexivity.
+    rewrite Heq by eauto.
+    reflexivity.
+  * simpl; lia.
+Qed.
+
+(* We need to know that [create] returns no longer list than it receives.
+   Like [fromDistinctAscList_create_preserves_length], just a few more cases.
+ *)
+Program Fixpoint fromList_create_preserves_length
+  i xs {measure (Z.to_nat i)} :
+  (1 <= i)%Z ->
+  forall (P : Map e a * list (e * a) * list (e * a) -> Prop),
+  ( forall s ys zs ,
+    (length ys <= length xs)%nat ->
+    P (s, ys, zs)
+  ) ->
+  P (fromList_create i xs) := _.
+Next Obligation.
+  intros.
+  rename fromList_create_preserves_length into IH.
+  rewrite fromList_create_eq by assumption.
+  unfold fromList_create_f.
+  destruct xs.
+  * apply H0. reflexivity.
+  * repeat replace (#1) with 1%Z by reflexivity.
+    unfold op_zeze__, Eq_Integer___, op_zeze____.
+    destruct (Z.eqb_spec i 1).
+    + destruct p. destruct_match.
+      - apply H0. simpl. lia.
+      - apply H0. simpl. lia.
+    + assert (Z.to_nat (Bits.shiftR i #1) < Z.to_nat i)%nat. {
+        apply Z2Nat.inj_lt.
+        apply Z.shiftr_nonneg. lia.
+        lia.
+        apply Z_shiftr_lt; lia.
+      }
+      apply IH.
+      - assumption. 
+      - apply Z_shiftr_pos; lia.
+      - intros.
+        destruct_match.
+        ** apply H0. simpl in *. lia.
+        ** apply IH.
+           -- assumption.
+           -- apply Z_shiftr_pos; lia.
+           -- intros.
+              repeat destruct_match.
+              ++ apply H0. simpl in *. lia.
+              ++ apply H0. simpl in *. lia.
+              ++ apply H0. simpl in *. lia.
+Qed.
+
+Lemma fromList_go_eq:
+  forall i s xs, (0 < i)%Z ->
+  fromList_go i s xs = fromList_go_f fromList_go i s xs.
+Proof.
+  intros.
+  change (deferredFix (fun g => uncurry (uncurry (fromList_go_f (curry (curry g))))) (i, s, xs) =
+    uncurry (uncurry (fromList_go_f fromList_go)) (i, s, xs)).
+  rewrite deferredFix_eq_on with
+    (P := fun p => (1 <= fst (fst p))%Z)
+    (R := fun x y => (length (snd x) < length (snd y))%nat); only 1: reflexivity.
+  * apply well_founded_ltof with (f := fun x => length (snd x)).
+  * intros g h p Px Heq.
+    destruct p as [[x y] z].
+    simpl in *.
+    unfold fromList_go_f.
+    destruct_match; try reflexivity.
+    eapply fromList_create_preserves_length; try lia.
+    intros s' ys zs Hlength.
+    destruct_match; try reflexivity.
+    destruct_match; try reflexivity.
+    destruct_match; try reflexivity.
+    destruct_match; try reflexivity.
+    apply Heq.
+    + apply Z_shiftl_pos.
+      lia.
+    + simpl. simpl in *. lia.
+  * simpl. lia.
+Qed.
+
+Program Fixpoint fromList_create_Desc
+  sz lb xs {measure (Z.to_nat sz)} :
+  (0 <= sz)%Z ->
+  not_ordered lb xs = false ->
+(*   StronglySorted (fun x y => x < y = true) (lb :: xs) -> *)
+  forall (P : Map e a * list (e * a) * list (e * a) -> Prop),
+  ( forall s ys zs,
+    Bounded s (Some lb) (safeHd ys) ->
+    isUB (safeHd ys) lb = true ->
+    xs = toList s ++ ys ++ zs->
+    ys = nil \/ (size s = (2*2^sz-1)%Z /\ zs = nil) ->
+    P (s, ys, zs)
+  ) ->
+  P (fromList_create (2^sz)%Z xs) := _.
+Next Obligation.
+  intros ???? Hnonneg HheadOrdered.
+  rename fromList_create_Desc into IH.
+  rewrite fromList_create_eq
+    by (enough (0 < 2^sz)%Z by lia; apply Z.pow_pos_nonneg; lia).
+  unfold fromList_create_f.
+  destruct xs.
+  * intros X HX. apply HX. clear HX.
+    - solve_Bounded.
+    - reflexivity.
+    - reflexivity.
+    - left. reflexivity.
+  * repeat replace (#1) with 1%Z by reflexivity.
+    unfold op_zeze__, Eq_Integer___, op_zeze____.
+    
+    simpl in HheadOrdered. destruct p.
+
+(*     assert (isUB (safeHd xs) e0 = true). {
+      destruct xs; try reflexivity.
+      inversion H5. assumption.
+    } *)
+
+    destruct (Z.eqb_spec (2^sz) 1); [ destruct_match | ].
+    - intros X HX. apply HX; clear HX.
+      ++ solve_Bounded.
+      ++ reflexivity.
+      ++ rewrite toList_Bin, toList_Tip, app_nil_r. reflexivity.
+      ++ left. reflexivity.
+    - intros X HX. apply HX; clear HX.
+      ++ destruct xs; simpl in Heq;  solve_Bounded. destruct p. unfold safeHd. unfold isUB. order e.
+      ++ destruct xs; simpl in *; solve_Bounds. destruct p. solve_Bounds.
+      ++ rewrite toList_Bin, toList_Tip, !app_nil_r, !app_nil_l. reflexivity.
+      ++ right. split. rewrite size_Bin. lia. reflexivity.
+    - assert (~ (sz = 0))%Z by (intro; subst; simpl in n; congruence).
+      assert (sz > 0)%Z by lia.
+      replace ((Bits.shiftR (2 ^ sz)%Z 1%Z)) with (2^(sz - 1))%Z.
+      Focus 2.
+        unfold Bits.shiftR, Bits.instance_Bits_Int.
+        rewrite Z.shiftr_div_pow2 by lia.
+        rewrite Z.pow_sub_r by lia.
+        reflexivity.
+      assert (Z.to_nat (sz - 1) < Z.to_nat sz)%nat.
+      { rewrite Z2Nat.inj_sub by lia. 
+        apply Nat.sub_lt.
+        apply Z2Nat.inj_le.
+        lia.
+        lia.
+        lia.
+        replace (Z.to_nat 1) with 1 by reflexivity.
+        lia.
+      }
+      eapply IH.
+      ++ assumption.
+      ++ lia.
+      ++ eassumption.
+      ++ intros l ys zs HBounded_l HisUB_l Hlist_l Hsize_l.
+         destruct ys.
+         + intros X HX. apply HX. clear HX.
+           ** solve_Bounded.
+           ** assumption.
+           ** assumption.
+           ** left; reflexivity.
+         + simpl in HBounded_l.
+           destruct Hsize_l as [? | [??]]; try congruence.
+           subst. rewrite app_nil_r in Hlist_l. destruct p.
+           assert (isLB (Some lb) e1 = true) by solve_Bounds.
+           destruct ys; only 2: destruct_match.
+           -- intros X HX. apply HX; clear HX.
+              ** assert (isUB None e1 = true) by reflexivity.
+                 applyDesc insertMax_Desc.
+              ** reflexivity.
+              ** erewrite toList_insertMax by eassumption.
+                 rewrite app_nil_l, <- app_assoc.
+                 assumption.
+              ** left; reflexivity.
+           -- intros X HX. apply HX; clear HX.
+              ** solve_Bounded.
+              ** reflexivity.
+              ** rewrite app_nil_l. simpl in Hlist_l.
+                 assumption.
+              ** left; reflexivity.
+           -- eapply IH; clear IH.
+              ** assumption.
+              ** lia.
+              ** eassumption.
+              ** simpl in Heq.
+                 intros r zs zs' HBounded_r HisUB_r Hlist_r Hsize_r.
+                 intros X HX. apply HX. clear HX.
+                 --- applyDesc link_Desc.
+                 --- solve_Bounds.
+                 --- erewrite toList_link by eassumption.
+                     rewrite Hlist_l. rewrite Hlist_r.
+                     rewrite <- !app_assoc.  reflexivity.
+                 --- destruct Hsize_r; [left; assumption| right].
+                     destruct H4.
+                     split; only 2: assumption.
+                     applyDesc link_Desc.
+                     replace (size l). rewrite H4.
+                     rewrite mul_pow_sub in * by lia.
+                     lia.
+Qed.
+
+Lemma foldl_foldl' : forall {b} f (x : b) (l: list (e * a)),
+  Foldable.foldl f x l = Foldable.foldl' f x l.
+Proof.
+  intros.  unfold Foldable.foldl, Foldable.foldl'; unfold Foldable.Foldable__list;
+    unfold  Foldable.foldl__ , Foldable.foldl'__ ; 
+    unfold Foldable.Foldable__list_foldl', Foldable.Foldable__list_foldl;
+    unfold Base.foldl, Base.foldl'. reflexivity.
+Qed.
+
+Definition fromList'' :=
+          fun (t0: Map e a) (xs: list (e * a)) =>
+            let ins :=
+              fun arg_2__ arg_3__ =>
+                match arg_2__, arg_3__ with
+                | t, pair k x => insert k x t
+                end in
+            Data.Foldable.foldl ins t0 xs.
+
+
+Lemma fromList'_fromList'': forall m l,
+  fromList' m l = fromList'' m l.
+Proof.
+  intros. unfold fromList'. unfold fromList''. rewrite <- (foldl_foldl' _ m l). reflexivity.
+Qed.
+
+Lemma fromList'_Desc:
+  forall s l,
+  Bounded s None None ->
+  Desc' (fromList' s l) None None (fun i => sem_for_lists (rev l) i ||| sem s i).
+Proof.
+  intros. rewrite fromList'_fromList''.
+  unfold fromList''.
+  rewrite Foldable.hs_coq_foldl_list.
+  revert s H.
+  induction l.
+  * intros.
+    simpl.
+    solve_Desc.
+  * intros.
+    simpl. destruct a0.
+    applyDesc insert_Desc.
+    applyDesc IHl.
+    solve_Desc. f_solver; rewrite sem_list_app in Heqo0.
+    + rewrite Heqo1 in Heqo0. inversion Heqo0. reflexivity.
+    + rewrite Heqo1 in Heqo0. inversion Heqo0. reflexivity.
+    + rewrite Heqo1 in Heqo0. simpl in Heqo0. rewrite Heqb in Heqo0. rewrite Hsem in Hsem0.
+      rewrite Hsem0 in Heqo0. assumption.
+    + rewrite Heqo1 in Heqo0. simpl in Heqo0. rewrite Heqb in Heqo0. inversion Heqo0.
+    + rewrite Heqo2 in Heqo0. inversion Heqo0.
+    + rewrite Heqo2 in Heqo0. inversion Heqo0.
+    + rewrite Heqo2 in Heqo0. simpl in Heqo0. rewrite Heqb in Heqo0. inversion Heqo0.
+    + rewrite Heqo2 in Heqo0. inversion Heqo0.
+    + rewrite Heqo2 in Heqo0. inversion Heqo0.
+    + rewrite Heqo2 in Heqo0. simpl in Heqo0. rewrite Heqb in Heqo0. inversion Heqo0.
+    + rewrite Heqo1 in Heqo0. simpl in Heqo0. rewrite Heqb in Heqo0. inversion Heqo0.
+Qed. 
+
+(*In a well formed map, we can only find each key once in the list, so it doesn't matter
+if we look in the list or the reverse list*)
+Lemma sem_toList_reverse: forall m lb ub i,
+  Bounded m lb ub ->
+  sem_for_lists (rev (toList m)) i = sem_for_lists (toList m) i.
+Proof.
+  intros. revert i. induction H; intros.
+  - simpl. reflexivity.
+  - rewrite toList_Bin. rewrite rev_app_distr. rewrite sem_list_app.
+    rewrite sem_list_app. simpl. rewrite sem_list_app. 
+    rewrite IHBounded2. simpl. rewrite IHBounded1. repeat (erewrite <- toList_sem'').
+    destruct (sem s2 i) eqn : ?. assert (sem s1 i = None). { eapply sem_outside_above.
+    apply H. unfold isUB. apply (sem_inside H0) in Heqo. destruct Heqo. order_Bounds. }
+    rewrite H5. simpl. assert (i == x = false) by solve_Bounds. rewrite H6. reflexivity.
+    simpl. destruct (i == x) eqn : ?. assert (sem s1 i = None). { eapply sem_outside_above.
+    apply H. unfold isUB. order_Bounds. } rewrite H5. simpl. reflexivity. simpl.
+    rewrite oro_None_r. reflexivity. apply H. apply H0.
+Qed.
+
+
+Program Fixpoint fromList_go_Desc
+  sz s xs {measure (length xs)} :
+  (0 <= sz)%Z ->
+  Bounded s None (safeHd xs) ->
+  xs = nil \/ size s = (2*2^sz-1)%Z ->
+  Desc' (fromList_go (2^sz)%Z s xs) None None
+    (fun i => sem_for_lists (rev xs) i ||| sem s i) := _.
+Next Obligation.
+  intros.
+  rename fromList_go_Desc into IH.
+  rewrite fromList_go_eq by (apply Z.pow_pos_nonneg; lia).
+  unfold fromList_go_f.
+  destruct xs as [ | ? [ | ?? ]].
+  * solve_Desc.
+  * destruct H1; try congruence.
+    simpl safeHd in *. destruct p.
+    assert (isUB None e0 = true) by reflexivity.
+    applyDesc insertMax_Desc.
+    solve_Desc. simpl.
+    (*setoid_rewrite elem_cons.*)
+    f_solver.
+  * destruct H1; try congruence.
+    repeat replace (#1) with 1%Z by reflexivity.
+    replace ((Bits.shiftL (2 ^ sz)%Z 1))%Z with (2 ^ (1 + sz))%Z.
+    Focus 2.
+      unfold Bits.shiftL, Bits.instance_Bits_Int.
+      rewrite Z.shiftl_mul_pow2 by lia.
+      rewrite Z.pow_add_r by lia.
+      lia. destruct p.
+    destruct_match.
+    --  apply Bounded_relax_ub_None in H0. 
+        applyDesc fromList'_Desc.
+        solve_Desc.
+    --  eapply fromList_create_Desc.
+        - lia.
+        - eassumption.
+        - intros.
+          subst.
+          simpl safeHd in *.
+
+          applyDesc link_Desc.
+          destruct zs.
+          ++  rewrite app_nil_r in H4.
+              eapply IH.
+              + rewrite H4. simpl. rewrite app_length. lia.
+              + lia.
+              + assumption.
+              + destruct H5 as [?|[??]]; [left; assumption | right].
+                replace (size s1). replace (size s).  replace (size s0).
+                rewrite Z.pow_add_r by lia.
+                lia.
+              + intros.
+                rewrite H4.
+                solve_Desc. simpl.
+                (*setoid_rewrite elem_cons.*)
+                setoid_rewrite sem_list_app. setoid_rewrite rev_app_distr.
+                setoid_rewrite sem_list_app. 
+                setoid_rewrite (sem_toList_reverse s0 _ _ _ H2). 
+                setoid_rewrite <- toList_sem''; only 2: eassumption. f_solver.
+                ** assert (sem s i = None). { eapply sem_outside_above. apply H0. solve_Bounds. }
+                   rewrite H9 in Hsem. simpl in Hsem. assert (i == e0 = false) by solve_Bounds.
+                   rewrite H10 in Hsem. simpl in Hsem. rewrite Hsem in H8. inversion H8; reflexivity.
+                ** simpl in Heqo2. destruct( i == e0) eqn : ?. simpl in Hsem. 
+                   assert (sem s i = None). { eapply sem_outside_above. apply H0.
+                   solve_Bounds. } rewrite H9 in Hsem. simpl in Hsem. rewrite Hsem in H8.
+                  rewrite Heqo2 in H8. inversion H8; reflexivity.
+                ** inversion Heqo2.
+                ** simpl in Heqo2. destruct (i == e0) eqn : ?. inversion Heqo2.
+                   simpl in Hsem. rewrite Hsem in H8. inversion H8.
+                ** destruct (sem s i); simpl in Hsem; inversion Hsem. rewrite H8 in H10.
+                   inversion H10. destruct (i == e0); simpl in Hsem; inversion Hsem.
+                    rewrite H8 in H11. inversion H11. rewrite H11 in H8. inversion H8.
+                ** simpl in Heqo2. destruct (i == e0) eqn : ?. simpl in Hsem.
+                   destruct (sem s i); simpl in Hsem. rewrite Hsem in H8. inversion H8.
+                    rewrite Hsem in H8; inversion H8. inversion Heqo2.
+         ++ destruct H5 as [ ? | [? Habsurd]]; try congruence.
+            subst. rewrite app_nil_l in H4.
+            rewrite H4.
+            apply Bounded_relax_ub_None in HB.
+            applyDesc fromList'_Desc.
+            solve_Desc. simpl.
+            (*setoid_rewrite elem_cons.*)
+            setoid_rewrite sem_list_app. setoid_rewrite rev_app_distr. simpl.
+            setoid_rewrite sem_list_app. setoid_rewrite (sem_toList_reverse s0 _ _ _ H2). 
+            setoid_rewrite <- toList_sem''; only 2: eassumption. simpl in Hsem0.
+            f_solver.
+            ** assert (sem s i = None). { eapply sem_outside_above. apply H0.
+              solve_Bounds. } rewrite H5 in Hsem. simpl in Hsem. 
+              assert (i == e0 = false) by solve_Bounds. rewrite H6 in Hsem. simpl in Hsem.
+              rewrite Hsem in Hsem0. inversion Hsem0; reflexivity.
+            **  assert (sem s i = None). { eapply sem_outside_above. apply H0.
+              solve_Bounds. } rewrite H5 in Hsem. simpl in Hsem. rewrite Hsem in Hsem0.
+              inversion Hsem0; reflexivity.
+            ** destruct (sem s i); simpl in Hsem; rewrite Hsem in Hsem0. inversion Hsem0.
+                destruct (i == e0); simpl in Hsem. inversion Hsem0. inversion Hsem0.
+            ** destruct (sem s i). simpl in Hsem. rewrite Hsem in Hsem0. inversion Hsem0.
+              simpl in Hsem. rewrite Hsem in Hsem0. inversion Hsem0.
+Qed.
+
+Lemma fromList_Desc:
+  forall xs,
+  Desc' (fromList xs) None None (fun i => sem_for_lists (rev xs) i).
+Proof.
+  intros.
+  cbv beta delta [fromList].
+  destruct xs as [ | ? [|??] ].
+  * solve_Desc.
+  * destruct p. solve_Desc.
+  * fold fromList'. destruct p.
+    zeta_one.
+    fold not_ordered.
+    zeta_one.
+    fold fromList_create_f.
+    fold fromList_create.
+    zeta_one.
+    fold fromList_go_f.
+    fold fromList_go.
+    zeta_one.
+    destruct_match.
+    - applyDesc fromList'_Desc.
+      solve_Desc. simpl. setoid_rewrite sem_list_app. setoid_rewrite sem_list_app.
+       simpl. destruct p0. simpl in Hsem. setoid_rewrite sem_list_app in Hsem. simpl in Hsem.
+      (*setoid_rewrite elem_cons.*)
+      f_solver.
+    - repeat replace (#1) with (2^0)%Z by reflexivity.
+      eapply fromList_go_Desc.
+      + lia.
+      + destruct p0. simpl in Heq. 
+        solve_Bounded.
+      + right. reflexivity.
+      + intros.
+        solve_Desc. simpl. setoid_rewrite sem_list_app. setoid_rewrite sem_list_app.
+        simpl. simpl in H1. setoid_rewrite sem_list_app in H1. simpl in H1.
+        f_solver.
+Qed.
