examples/containers/theories/MapProofs/MapFunctionProofs.v
@@ -1,0 +1,268 @@
+Require Import GHC.Base.
+Import GHC.Base.Notations.
+Require Import Proofs.GHC.Base.
+Require Import Data.Map.Internal.
+Import GHC.Num.Notations.
+Require Import OrdTactic.
+Require Import Psatz.
+Require Import Tactics.
+Set Bullet Behavior "Strict Subproofs".
+Require Import MapProofs.Bounds.
+Require Import MapProofs.ContainerAxiomsProofs.
+Require Import MapProofs.UnionIntersectDifferenceProofs.
+(** ** Verification of [map] *)
+
+(*Note: for map_spec, the definition we want is not provable:
+[(forall i v, sem m i = Some v <-> sem (mapWithKey f m) i = Some (f i v))]
+
+This is because of three problems
+1. Even if two keys k1 and k2 are equal (k1 == k2), this does not guarantee
+   that (f k = f k2).
+2. We cannot compare the results using Haskell equality because neither a not b
+   are required to be members of Eq.
+3. If f is not injective, then the (<-) is clearly not true (for example, 
+   suppose f = \x -> \y -> 1)
+
+This is not an issue in SetProofs because [Ord b] is a necessary condition for the input and the
+map function is defined very differently, leading to an entirely different specification.
+
+There are two solutions to this: 
+1. Require that if k == k1 and v == v1, then f k v = f k1 v1, which is not true in general
+2. Require that [a] and [b] be members of [Eq], which is also not true in general. We also must
+   require that k1 == k2 and v1 == v2 -> f k1 v1 == f k2 v2, which should be true in all cases, since
+   this is the definition of a pure function in Haskell.
+
+Both cases are proved below. We prove both cases because it could happen that Haskell equality agrees
+with Coq equality on the values but the values are not an instance of [Ord] (and this will be used in
+[FMapInterface]
+
+*)
+
+(*Specification using Coq equality*)
+
+(*The same keys are in both maps*)
+Lemma map_none_spec:
+  forall {b} {a} {e} `{Eq_ e} `{Ord e} (f: e -> a -> b) (m: Map e a) lb ub,
+  Bounded m lb ub ->
+  (forall i, sem m i = None <-> sem (mapWithKey f m) i = None).
+Proof.
+  intros. generalize dependent i. induction H2; intros; split; intros.
+  - reflexivity.
+  - reflexivity.
+  - simpl. simpl in H6. destruct (sem s1 i) eqn : ?. inversion H6. 
+    apply IHBounded1 in Heqo. rewrite Heqo. simpl. simpl in H6.
+    destruct (i == x) eqn : ?. inversion H6. simpl. simpl in H6.
+    apply IHBounded2. apply H6.
+  - simpl in H6. simpl. destruct (sem (mapWithKey f s1) i) eqn : ?. inversion H6.
+    apply IHBounded1 in Heqo. rewrite Heqo. simpl. destruct (i == x) eqn : ?. inversion H6.
+    simpl. simpl in H6. apply IHBounded2. apply H6.
+Qed. 
+
+(*Says that if we take any (key, value) pair in the map resulting from mapWithKey, then they
+come from a corresponding entry in the original map*)
+Lemma map_spec_reverse : 
+  forall {b} {a} {t}  `{Ord t} (H : EqLaws t) (f : t -> a -> b) (m : Map t a) lb ub,
+  Bounded m lb ub ->
+  (forall k k2 v v2, k == k2 = true -> v = v2 -> f k v = f k2 v2) ->
+  (forall i v, sem (mapWithKey f m) i = Some v -> exists value, sem m i = Some value /\ v = f i value).
+Proof.
+  intros. generalize dependent i. generalize dependent v. induction H2; intros.
+  - simpl in H4. inversion H4.
+  - simpl in H7. simpl. destruct ( sem (mapWithKey f s1) i ) eqn : ?. apply IHBounded1 in Heqo.
+    destruct Heqo. exists x0. destruct H8. rewrite H8. simpl. split. reflexivity. inversion H7; subst.
+    reflexivity. simpl in H7.  assert (sem s1 i = None). { erewrite map_none_spec. apply Heqo. apply H2_. }
+    rewrite H8. destruct (i == x) eqn : ?. simpl in H7. simpl. exists v. split. reflexivity. inversion H7. 
+    apply H3. apply Eq_Symmetric. apply Heqb0. reflexivity. simpl. inversion H7. apply IHBounded2.
+    assumption.
+Qed.
+
+(*If (k,v) is in the original map, then (k, f k v) is in the new map*)
+Lemma map_spec_coq:
+  forall {b} {a} {e} `{Ord e} (H: EqLaws e) (f : e -> a -> b) (m : Map e a) lb ub,
+  Bounded m lb ub ->
+  (forall k k2 v v2, k == k2 = true -> v = v2 -> f k v = f k2 v2) ->
+  (forall i v, sem m i = Some v -> sem (mapWithKey f m) i = Some (f i v)).
+Proof.
+  intros.  generalize dependent i. generalize dependent v. induction H2; intros.
+  - inversion H4.
+  - simpl. simpl in H7. destruct (sem s1 i) eqn : ?.
+    * apply IHBounded1 in Heqo. rewrite Heqo. simpl. inversion H7; subst; reflexivity.
+    * assert (sem (mapWithKey f s1) i = None). { erewrite <- map_none_spec. assumption. apply H2_. }
+      simpl in H7. rewrite H8. simpl. destruct (i == x) eqn : ?.
+      + simpl. simpl in H7. inversion H7; subst. erewrite H3. reflexivity. apply Eq_Symmetric.
+        apply Heqb0. reflexivity.
+      + simpl. apply IHBounded2. simpl in H7. assumption.
+Qed.
+
+(*If f is injective, then (k,v) is in the original map iff (k, f k v) is in the new map*)
+Lemma map_spec_coq_injective:
+  forall {b} {a} {e} `{Ord e} (H: EqLaws e) (f : e -> a -> b) (m : Map e a) lb ub,
+  Bounded m lb ub ->
+  (forall k k2 v v2, k == k2 = true -> v = v2 -> f k v = f k2 v2) ->
+  (forall k k2 v v2, f k v = f k2 v2 -> k == k2 = true /\ v = v2) ->
+  (forall i v, sem m i = Some v <-> sem (mapWithKey f m) i = Some (f i v)).
+Proof.
+  intros. split.
+  - intros. eapply map_spec_coq; eassumption.
+  - generalize dependent i. generalize dependent v. induction H2; intros.
+    + inversion H2.
+    + simpl in H8. simpl. destruct (sem (mapWithKey f s1) i) eqn : ?.
+      * assert (A:= Heqo). eapply map_spec_reverse in Heqo. destruct Heqo.
+        destruct H9. subst. inversion H8. rewrite H9. simpl.
+        apply H4 in H10. destruct H10. subst. reflexivity. assumption. apply H2_.
+        apply H3.
+      * rewrite <- map_none_spec in Heqo. rewrite Heqo. simpl. simpl in H8. destruct (i == x) eqn : ?.
+        -- simpl. simpl in H8. inversion H8. apply H4 in H10. destruct H10; subst; reflexivity.
+        -- simpl in H8. simpl. apply IHBounded2. assert (A:= H8). eapply map_spec_reverse in H8.
+           assumption. assumption. apply H2_0. assumption.
+        -- apply H2_.
+Qed.
+
+(*Specification using Haskell Equality. This requires several lemmas to replace the use
+of [subst] and [rewrite].*)
+
+(*Haskell equality version of [oro_Some_l]*)
+Lemma sem_haskell_eq_some : forall {a} {b} `{EqLaws a} `{EqLaws b} (a1: a) (m : Map a b) b1 o,
+  sem m a1 == Some b1 = true ->
+  (sem m a1 ||| o) == Some b1 = true.
+Proof.
+  intros. destruct (sem m a1) eqn : ?.
+  - simpl. assumption.
+  - inversion H3.
+Qed.
+
+(*Haskell equality version of [oro_None_l]*)
+Lemma sem_haskell_eq_none: forall {a} {b} `{EqLaws a} `{EqLaws b} (a1: a) (m : Map a b) o,
+  sem m a1 == None = true ->
+  (sem m a1 ||| o) == o = true.
+Proof.
+  intros. destruct (sem m a1) eqn : ?.
+  - inversion H3.
+  - simpl. apply Eq_Reflexive.
+Qed.
+
+(*Haskell equality version of [map_none_spec] *)
+Lemma map_none_spec_haskell:
+  forall {b} {a} {e} `{Ord e} (H : EqLaws e) `{EqLaws a} `{EqLaws b} (f: e -> a -> b) (m: Map e a) lb ub,
+  Bounded m lb ub ->
+  (forall i, sem m i == None = true <-> sem (mapWithKey f m) i == None = true).
+Proof.
+  intros. generalize dependent i. induction H6; intros; split; intros.
+  - simpl. apply Eq_Reflexive. 
+  - simpl. apply Eq_Reflexive. 
+  - simpl. simpl in H10. destruct (sem s1 i) eqn : ?. simpl in H10. inversion H10. simpl in H10.
+    destruct (i == x) eqn : ?. simpl in H10. inversion H10. simpl in H10. destruct (sem s2 i) eqn : ?.
+    inversion H10. apply eq_coq_implies_haskell in Heqo. apply eq_coq_implies_haskell in Heqo0.
+    apply IHBounded1 in Heqo. apply IHBounded2 in Heqo0. rewrite  oro_assoc. simpl.
+    apply (sem_haskell_eq_none _  _ (sem (mapWithKey f s2) i)) in Heqo.
+    eapply Eq_Transitive. apply Heqo. apply Heqo0.
+  - simpl. simpl in H10. destruct (sem (mapWithKey f s1) i) eqn : ?. inversion H10.
+    destruct (i == x) eqn : ?. inversion H10. destruct (sem (mapWithKey f s2) i) eqn : ?.
+    inversion H10. apply eq_coq_implies_haskell in Heqo. apply eq_coq_implies_haskell in Heqo0.
+    simpl. rewrite oro_assoc. simpl. apply IHBounded1 in Heqo. apply IHBounded2 in Heqo0.
+    apply (sem_haskell_eq_none  _ _  (sem s2 i)) in Heqo. eapply Eq_Transitive.
+    apply Heqo. apply Heqo0.
+Qed.
+
+(*Haskell equality version of [map_spec_reverse]*)
+Lemma map_spec_haskell_reverse : 
+  forall {b} {a} {t}  `{Ord t} (H : EqLaws t) `{EqLaws b} `{EqLaws a}
+   (f : t -> a -> b) (m : Map t a) lb ub,
+  Bounded m lb ub ->
+  (forall x1 x2 y1 y2, x1 == x2 = true -> y1 == y2 = true -> f x1 y1 == f x2 y2 = true) ->
+  (forall i v, sem (mapWithKey f m) i == Some v = true -> 
+    exists value, sem m i == Some value = true /\ v == f i value = true).
+Proof.
+  intros.
+  generalize dependent i. generalize dependent v. induction H6; intros.
+  - inversion H8.
+  - simpl in H11. simpl. destruct (sem (mapWithKey f s1) i) eqn : ?.
+    + assert ( _GHC.Base.==_ (sem (mapWithKey f s1) i) (Some b0) = true). { rewrite Heqo.
+      apply Eq_Reflexive. } apply IHBounded1 in H12. destruct H12. exists x0.
+      destruct H12. split. rewrite oro_assoc. apply sem_haskell_eq_some. 
+      apply H12. simpl in H11. rewrite simpl_option_some_eq in H11. eapply Eq_Transitive.
+      apply Eq_Symmetric. apply H11. apply H13.
+    + simpl in H11. apply eq_coq_implies_haskell in Heqo. rewrite <- map_none_spec_haskell in Heqo.
+      destruct (sem s1 i). inversion Heqo. simpl. destruct (i == x) eqn : ?. simpl in H11.
+      simpl. exists v. split. apply Eq_Reflexive. rewrite simpl_option_some_eq in H11. 
+      assert ((f x v) == (f i v) = true). { apply H7. apply Eq_Symmetric. apply Heqb0. 
+      apply Eq_Reflexive. } eapply Eq_Transitive. apply Eq_Symmetric. apply H11. apply H12.
+      simpl. simpl in H11. apply IHBounded2 in H11. apply H11. apply H1. apply H5. apply H3.
+      apply H6_.
+Qed. 
+
+(*A substitute for [rewrite]: If we know a1 == a3, and we have a1 == a2 in the goal, 
+we can prove a2 == a3 instead*)
+Lemma rewrite_eq_haskell : forall {a} `{EqLaws a} a1 a2 a3,
+  a1 == a2 = true -> (a1 == a3 = true <-> a2 == a3 = true).
+Proof.
+  intros; split; intros.
+  - eapply Eq_Transitive. apply Eq_Symmetric. apply H1. apply H2.
+  - eapply Eq_Transitive. apply H1. apply H2.
+Qed.
+
+(*Specification for mapWithKey using Haskell equality*)
+Lemma map_spec_haskell:
+  forall {b} {a} {e} `{Ord e} (H: EqLaws e) `{EqLaws b} `{EqLaws a} (f : e -> a -> b) (m : Map e a) lb ub,
+  Bounded m lb ub ->
+  (forall x1 x2 y1 y2, x1 == x2 = true -> y1 == y2 = true -> f x1 y1 == f x2 y2 = true) ->
+  (forall i v, sem m i == Some v = true -> sem (mapWithKey f m) i == Some (f i v) = true).
+Proof.
+  intros.  generalize dependent i. generalize dependent v. induction H6; intros.
+  - inversion H8.
+  - simpl. simpl in H11. destruct (sem s1 i) eqn : ?.
+    * apply eq_coq_implies_haskell in Heqo. apply IHBounded1 in Heqo. rewrite oro_assoc.
+      eapply sem_haskell_eq_some. simpl in H11. rewrite simpl_option_some_eq in H11.
+      assert (f i a0 == f i v0 = true). { apply H7. apply Eq_Reflexive. apply H11. }
+      eapply Eq_Transitive. apply Heqo. rewrite simpl_option_some_eq. apply H12.
+    * apply eq_coq_implies_haskell in Heqo. erewrite map_none_spec_haskell in Heqo.
+      rewrite oro_assoc. eapply (sem_haskell_eq_none i (mapWithKey f s1)
+      (SomeIf (_GHC.Base.==_ i x) (f x v) ||| sem (mapWithKey f s2) i)) in Heqo.
+      (*rewrite to make the goal simpler*)
+      assert (_GHC.Base.==_ (sem (mapWithKey f s1) i ||| 
+      (SomeIf (_GHC.Base.==_ i x) (f x v) ||| sem (mapWithKey f s2) i))
+      (Some (f i v0)) = true <-> ((SomeIf (_GHC.Base.==_ i x) (f x v) ||| 
+      sem (mapWithKey f s2) i) == Some (f i v0) = true)).
+      apply rewrite_eq_haskell. apply Heqo. rewrite H12. clear H12.
+      destruct (i == x) eqn : ?. simpl. simpl in H11. rewrite simpl_option_some_eq.
+      apply H7. apply Eq_Symmetric. apply Heqb0. rewrite simpl_option_some_eq in H11. apply H11.
+      simpl. apply IHBounded2. simpl in H11. apply H11. assumption. assumption. assumption.
+      apply H6_.
+Qed.
+
+(*Once again. if f is injective, we get a stronger claim*)
+Lemma map_spec_haskell_injective:
+  forall {b} {a} {e} `{Ord e} (H: EqLaws e) `{EqLaws b} `{EqLaws a} (f : e -> a -> b) (m : Map e a) lb ub,
+  Bounded m lb ub ->
+  (forall x1 x2 y1 y2, x1 == x2 = true -> y1 == y2 = true -> f x1 y1 == f x2 y2 = true) ->
+  (forall k k2 v v2, f k v == f k2 v2 = true -> k == k2 = true /\ v = v2) ->
+  (forall i v, sem m i == Some v = true <-> sem (mapWithKey f m) i == Some (f i v) = true).
+Proof.
+  intros. split.
+  - intros. eapply map_spec_haskell; eassumption.
+  - generalize dependent i. generalize dependent v. induction H6; intros.
+    + inversion H6.
+    + simpl in H12. simpl. destruct (sem (mapWithKey f s1) i) eqn : ?.
+      * assert (A:= Heqo). apply eq_coq_implies_haskell in Heqo. eapply map_spec_haskell_reverse in Heqo.
+        destruct Heqo. destruct H13. simpl in H12. 
+        apply eq_coq_implies_haskell in A. assert ( (sem (mapWithKey f s1) i) == (Some (f i v0)) = true).
+        { eapply Eq_Transitive. apply A. apply H12. } apply IHBounded1 in H15.
+         rewrite oro_assoc. eapply sem_haskell_eq_some. apply H15. assumption. assumption.
+        apply H5. apply H6_. assumption.
+      * apply eq_coq_implies_haskell in Heqo. rewrite <- map_none_spec_haskell in Heqo.
+        destruct (sem s1 i). inversion Heqo. simpl. simpl in H12. destruct (i== x) eqn : ?.
+        -- simpl. simpl in H12. apply H8 in H12. destruct H12; subst; apply Eq_Reflexive.
+        -- simpl. simpl in H12. apply IHBounded2. apply H12.
+        -- assumption.
+        -- apply H5.
+        -- assumption.
+        -- apply H6_.
+Qed.
+
+Lemma map_no_key_spec :  forall {e} {a} {b} `{Ord e} (f : a -> b) (m : Map e a),
+  Internal.map f m = mapWithKey (fun k v => f v) m.
+Proof.
+  intros. induction m.
+  - simpl. rewrite IHm1. rewrite IHm2. reflexivity.
+  - simpl. reflexivity.
+Qed.
